big changes to frontend, now i can get ENS to compile. however, i am going to need to relax the conditions on instruction validity, which may complicate proofs

elle/generated/FourL.ml
@@ -1,23 +1,126 @@
 module FourL : sig
+  type char
   val compiler : string -> string option
 end = struct
 
-type int = Int_of_integer of Big_int.big_int;;
-
 type num = One | Bit0 of num | Bit1 of num;;
 
-let one_inta : int = Int_of_integer (Big_int.big_int_of_int 1);;
+let rec equal_num x0 x1 = match x0, x1 with Bit0 x2, Bit1 x3 -> false
+                    | Bit1 x3, Bit0 x2 -> false
+                    | One, Bit1 x3 -> false
+                    | Bit1 x3, One -> false
+                    | One, Bit0 x2 -> false
+                    | Bit0 x2, One -> false
+                    | Bit1 x3, Bit1 y3 -> equal_num x3 y3
+                    | Bit0 x2, Bit0 y2 -> equal_num x2 y2
+                    | One, One -> true;;
+
+type int = Zero_int | Pos of num | Neg of num;;
+
+let rec equal_inta x0 x1 = match x0, x1 with Neg k, Neg l -> equal_num k l
+                     | Neg k, Pos l -> false
+                     | Neg k, Zero_int -> false
+                     | Pos k, Neg l -> false
+                     | Pos k, Pos l -> equal_num k l
+                     | Pos k, Zero_int -> false
+                     | Zero_int, Neg l -> false
+                     | Zero_int, Pos l -> false
+                     | Zero_int, Zero_int -> true;;
+
+type 'a equal = {equal : 'a -> 'a -> bool};;
+let equal _A = _A.equal;;
+
+let equal_int = ({equal = equal_inta} : int equal);;
+
+let one_inta : int = Pos One;;
 
 type 'a one = {one : 'a};;
 let one _A = _A.one;;
 
 let one_int = ({one = one_inta} : int one);;
 
-let rec integer_of_int (Int_of_integer k) = k;;
+let rec plus_num
+  x0 x1 = match x0, x1 with Bit1 m, Bit1 n -> Bit0 (plus_num (plus_num m n) One)
+    | Bit1 m, Bit0 n -> Bit1 (plus_num m n)
+    | Bit1 m, One -> Bit0 (plus_num m One)
+    | Bit0 m, Bit1 n -> Bit1 (plus_num m n)
+    | Bit0 m, Bit0 n -> Bit0 (plus_num m n)
+    | Bit0 m, One -> Bit1 m
+    | One, Bit1 n -> Bit0 (plus_num n One)
+    | One, Bit0 n -> Bit1 n
+    | One, One -> Bit0 One;;
 
-let rec times_inta
-  k l = Int_of_integer
-          (Big_int.mult_big_int (integer_of_int k) (integer_of_int l));;
+let rec uminus_int = function Neg m -> Pos m
+                     | Pos m -> Neg m
+                     | Zero_int -> Zero_int;;
+
+let rec bitM = function One -> One
+               | Bit0 n -> Bit1 (bitM n)
+               | Bit1 n -> Bit1 (Bit0 n);;
+
+let rec dup = function Neg n -> Neg (Bit0 n)
+              | Pos n -> Pos (Bit0 n)
+              | Zero_int -> Zero_int;;
+
+let rec plus_inta k l = match k, l with Neg m, Neg n -> Neg (plus_num m n)
+                    | Neg m, Pos n -> sub n m
+                    | Pos m, Neg n -> sub m n
+                    | Pos m, Pos n -> Pos (plus_num m n)
+                    | Zero_int, l -> l
+                    | k, Zero_int -> k
+and sub
+  x0 x1 = match x0, x1 with Bit0 m, Bit1 n -> minus_int (dup (sub m n)) one_inta
+    | Bit1 m, Bit0 n -> plus_inta (dup (sub m n)) one_inta
+    | Bit1 m, Bit1 n -> dup (sub m n)
+    | Bit0 m, Bit0 n -> dup (sub m n)
+    | One, Bit1 n -> Neg (Bit0 n)
+    | One, Bit0 n -> Neg (bitM n)
+    | Bit1 m, One -> Pos (Bit0 m)
+    | Bit0 m, One -> Pos (bitM m)
+    | One, One -> Zero_int
+and minus_int k l = match k, l with Neg m, Neg n -> sub n m
+                | Neg m, Pos n -> Neg (plus_num m n)
+                | Pos m, Neg n -> Pos (plus_num m n)
+                | Pos m, Pos n -> sub m n
+                | Zero_int, l -> uminus_int l
+                | k, Zero_int -> k;;
+
+type 'a plus = {plus : 'a -> 'a -> 'a};;
+let plus _A = _A.plus;;
+
+let plus_int = ({plus = plus_inta} : int plus);;
+
+type 'a zero = {zero : 'a};;
+let zero _A = _A.zero;;
+
+let zero_int = ({zero = Zero_int} : int zero);;
+
+type 'a semigroup_add = {plus_semigroup_add : 'a plus};;
+
+type 'a numeral =
+  {one_numeral : 'a one; semigroup_add_numeral : 'a semigroup_add};;
+
+let semigroup_add_int = ({plus_semigroup_add = plus_int} : int semigroup_add);;
+
+let numeral_int =
+  ({one_numeral = one_int; semigroup_add_numeral = semigroup_add_int} :
+    int numeral);;
+
+let rec times_num
+  m n = match m, n with
+    Bit1 m, Bit1 n -> Bit1 (plus_num (plus_num m n) (Bit0 (times_num m n)))
+    | Bit1 m, Bit0 n -> Bit0 (times_num (Bit1 m) n)
+    | Bit0 m, Bit1 n -> Bit0 (times_num m (Bit1 n))
+    | Bit0 m, Bit0 n -> Bit0 (Bit0 (times_num m n))
+    | One, n -> n
+    | m, One -> m;;
+
+let rec times_inta k l = match k, l with Neg m, Neg n -> Pos (times_num m n)
+                     | Neg m, Pos n -> Neg (times_num m n)
+                     | Pos m, Neg n -> Neg (times_num m n)
+                     | Pos m, Pos n -> Pos (times_num m n)
+                     | Zero_int, l -> Zero_int
+                     | k, Zero_int -> Zero_int;;
 
 type 'a times = {times : 'a -> 'a -> 'a};;
 let times _A = _A.times;;
@@ -28,51 +131,240 @@ let times_int = ({times = times_inta} : int times);;
 
 let power_int = ({one_power = one_int; times_power = times_int} : int power);;
 
-type 'a equal = {equal : 'a -> 'a -> bool};;
-let equal _A = _A.equal;;
+let rec less_eq_num x0 n = match x0, n with Bit1 m, Bit0 n -> less_num m n
+                      | Bit1 m, Bit1 n -> less_eq_num m n
+                      | Bit0 m, Bit1 n -> less_eq_num m n
+                      | Bit0 m, Bit0 n -> less_eq_num m n
+                      | Bit1 m, One -> false
+                      | Bit0 m, One -> false
+                      | One, n -> true
+and less_num m x1 = match m, x1 with Bit1 m, Bit0 n -> less_num m n
+               | Bit1 m, Bit1 n -> less_num m n
+               | Bit0 m, Bit1 n -> less_eq_num m n
+               | Bit0 m, Bit0 n -> less_num m n
+               | One, Bit1 n -> true
+               | One, Bit0 n -> true
+               | m, One -> false;;
 
-let equal_char = ({equal = (fun a b -> ((a : char) = b))} : char equal);;
+let rec less_eq_int x0 x1 = match x0, x1 with Neg k, Neg l -> less_eq_num l k
+                      | Neg k, Pos l -> true
+                      | Neg k, Zero_int -> true
+                      | Pos k, Neg l -> false
+                      | Pos k, Pos l -> less_eq_num k l
+                      | Pos k, Zero_int -> false
+                      | Zero_int, Neg l -> false
+                      | Zero_int, Pos l -> true
+                      | Zero_int, Zero_int -> true;;
 
-type nat = Nat of Big_int.big_int;;
+type 'a ord = {less_eq : 'a -> 'a -> bool; less : 'a -> 'a -> bool};;
+let less_eq _A = _A.less_eq;;
+let less _A = _A.less;;
+
+let rec less_int x0 x1 = match x0, x1 with Neg k, Neg l -> less_num l k
+                   | Neg k, Pos l -> true
+                   | Neg k, Zero_int -> true
+                   | Pos k, Neg l -> false
+                   | Pos k, Pos l -> less_num k l
+                   | Pos k, Zero_int -> false
+                   | Zero_int, Neg l -> false
+                   | Zero_int, Pos l -> true
+                   | Zero_int, Zero_int -> false;;
+
+let ord_int = ({less_eq = less_eq_int; less = less_int} : int ord);;
+
+type 'a ab_semigroup_add = {semigroup_add_ab_semigroup_add : 'a semigroup_add};;
+
+type 'a semigroup_mult = {times_semigroup_mult : 'a times};;
+
+type 'a semiring =
+  {ab_semigroup_add_semiring : 'a ab_semigroup_add;
+    semigroup_mult_semiring : 'a semigroup_mult};;
+
+let ab_semigroup_add_int =
+  ({semigroup_add_ab_semigroup_add = semigroup_add_int} :
+    int ab_semigroup_add);;
+
+let semigroup_mult_int =
+  ({times_semigroup_mult = times_int} : int semigroup_mult);;
+
+let semiring_int =
+  ({ab_semigroup_add_semiring = ab_semigroup_add_int;
+     semigroup_mult_semiring = semigroup_mult_int}
+    : int semiring);;
+
+type 'a preorder = {ord_preorder : 'a ord};;
+
+type 'a order = {preorder_order : 'a preorder};;
+
+let preorder_int = ({ord_preorder = ord_int} : int preorder);;
+
+let order_int = ({preorder_order = preorder_int} : int order);;
+
+type 'a mult_zero = {times_mult_zero : 'a times; zero_mult_zero : 'a zero};;
+
+let mult_zero_int =
+  ({times_mult_zero = times_int; zero_mult_zero = zero_int} : int mult_zero);;
+
+type 'a monoid_add =
+  {semigroup_add_monoid_add : 'a semigroup_add; zero_monoid_add : 'a zero};;
+
+type 'a comm_monoid_add =
+  {ab_semigroup_add_comm_monoid_add : 'a ab_semigroup_add;
+    monoid_add_comm_monoid_add : 'a monoid_add};;
+
+type 'a semiring_0 =
+  {comm_monoid_add_semiring_0 : 'a comm_monoid_add;
+    mult_zero_semiring_0 : 'a mult_zero; semiring_semiring_0 : 'a semiring};;
+
+let monoid_add_int =
+  ({semigroup_add_monoid_add = semigroup_add_int; zero_monoid_add = zero_int} :
+    int monoid_add);;
+
+let comm_monoid_add_int =
+  ({ab_semigroup_add_comm_monoid_add = ab_semigroup_add_int;
+     monoid_add_comm_monoid_add = monoid_add_int}
+    : int comm_monoid_add);;
+
+let semiring_0_int =
+  ({comm_monoid_add_semiring_0 = comm_monoid_add_int;
+     mult_zero_semiring_0 = mult_zero_int; semiring_semiring_0 = semiring_int}
+    : int semiring_0);;
+
+type 'a monoid_mult =
+  {semigroup_mult_monoid_mult : 'a semigroup_mult;
+    power_monoid_mult : 'a power};;
+
+type 'a semiring_numeral =
+  {monoid_mult_semiring_numeral : 'a monoid_mult;
+    numeral_semiring_numeral : 'a numeral;
+    semiring_semiring_numeral : 'a semiring};;
+
+type 'a zero_neq_one =
+  {one_zero_neq_one : 'a one; zero_zero_neq_one : 'a zero};;
+
+type 'a semiring_1 =
+  {semiring_numeral_semiring_1 : 'a semiring_numeral;
+    semiring_0_semiring_1 : 'a semiring_0;
+    zero_neq_one_semiring_1 : 'a zero_neq_one};;
+
+let monoid_mult_int =
+  ({semigroup_mult_monoid_mult = semigroup_mult_int;
+     power_monoid_mult = power_int}
+    : int monoid_mult);;
+
+let semiring_numeral_int =
+  ({monoid_mult_semiring_numeral = monoid_mult_int;
+     numeral_semiring_numeral = numeral_int;
+     semiring_semiring_numeral = semiring_int}
+    : int semiring_numeral);;
+
+let zero_neq_one_int =
+  ({one_zero_neq_one = one_int; zero_zero_neq_one = zero_int} :
+    int zero_neq_one);;
+
+let semiring_1_int =
+  ({semiring_numeral_semiring_1 = semiring_numeral_int;
+     semiring_0_semiring_1 = semiring_0_int;
+     zero_neq_one_semiring_1 = zero_neq_one_int}
+    : int semiring_1);;
+
+type 'a linorder = {order_linorder : 'a order};;
+
+let linorder_int = ({order_linorder = order_int} : int linorder);;
+
+type nat = Zero_nat | Suc of nat;;
+
+let rec equal_nata x0 x1 = match x0, x1 with Zero_nat, Suc x2 -> false
+                     | Suc x2, Zero_nat -> false
+                     | Suc x2, Suc y2 -> equal_nata x2 y2
+                     | Zero_nat, Zero_nat -> true;;
+
+let equal_nat = ({equal = equal_nata} : nat equal);;
+
+let rec less_eq_nat x0 n = match x0, n with Suc m, n -> less_nat m n
+                      | Zero_nat, n -> true
+and less_nat m x1 = match m, x1 with m, Suc n -> less_eq_nat m n
+               | n, Zero_nat -> false;;
+
+let ord_nat = ({less_eq = less_eq_nat; less = less_nat} : nat ord);;
+
+let rec eq _A a b = equal _A a b;;
+
+let rec equal_lista _A
+  x0 x1 = match x0, x1 with [], x21 :: x22 -> false
+    | x21 :: x22, [] -> false
+    | x21 :: x22, y21 :: y22 -> eq _A x21 y21 && equal_lista _A x22 y22
+    | [], [] -> true;;
+
+let rec equal_list _A = ({equal = equal_lista _A} : ('a list) equal);;
+
+let rec equal_bool p pa = match p, pa with p, true -> p
+                     | p, false -> not p
+                     | true, p -> p
+                     | false, p -> not p;;
+
+type char = Chara of bool * bool * bool * bool * bool * bool * bool * bool;;
+
+let rec equal_chara
+  (Chara (x1, x2, x3, x4, x5, x6, x7, x8))
+    (Chara (y1, y2, y3, y4, y5, y6, y7, y8)) =
+    equal_bool x1 y1 &&
+      (equal_bool x2 y2 &&
+        (equal_bool x3 y3 &&
+          (equal_bool x4 y4 &&
+            (equal_bool x5 y5 &&
+              (equal_bool x6 y6 && (equal_bool x7 y7 && equal_bool x8 y8))))));;
+
+let equal_char = ({equal = equal_chara} : char equal);;
 
 type 'a itself = Type;;
 
 type 'a len0 = {len_of : 'a itself -> nat};;
 let len_of _A = _A.len_of;;
 
-let rec integer_of_nat (Nat x) = x;;
+let rec plus_nat x0 n = match x0, n with Suc m, n -> plus_nat m (Suc n)
+                   | Zero_nat, n -> n;;
 
-let rec times_nat
-  m n = Nat (Big_int.mult_big_int (integer_of_nat m) (integer_of_nat n));;
+let rec times_nat x0 n = match x0, n with Zero_nat, n -> Zero_nat
+                    | Suc m, n -> plus_nat n (times_nat m n);;
 
-type 'a ord = {less_eq : 'a -> 'a -> bool; less : 'a -> 'a -> bool};;
-let less_eq _A = _A.less_eq;;
-let less _A = _A.less;;
+let one_nat : nat = Suc Zero_nat;;
 
-let rec max _A a b = (if less_eq _A a b then b else a);;
-
-let ord_integer =
-  ({less_eq = Big_int.le_big_int; less = Big_int.lt_big_int} :
-    Big_int.big_int ord);;
-
-let rec nat_of_integer k = Nat (max ord_integer Big_int.zero_big_int k);;
+let rec nat_of_num
+  = function Bit1 n -> (let m = nat_of_num n in Suc (plus_nat m m))
+    | Bit0 n -> (let m = nat_of_num n in plus_nat m m)
+    | One -> one_nat;;
 
 type 'a finite = unit;;
 
 type 'a bit0 = Abs_bit0 of int;;
 
-let rec len_of_bit0 _A
-  uu = times_nat (nat_of_integer (Big_int.big_int_of_int 2)) (len_of _A Type);;
+let rec len_of_bit0 _A uu = times_nat (nat_of_num (Bit0 One)) (len_of _A Type);;
 
 let rec len0_bit0 _A = ({len_of = len_of_bit0 _A} : 'a bit0 len0);;
 
-let one_nat : nat = Nat (Big_int.big_int_of_int 1);;
+type 'a bit1 = Abs_bit1 of int;;
+
+let rec len_of_bit1 _A
+  uu = plus_nat (times_nat (nat_of_num (Bit0 One)) (len_of _A Type)) one_nat;;
+
+let rec len0_bit1 _A = ({len_of = len_of_bit1 _A} : 'a bit1 len0);;
 
 type num1 = One_num1;;
 
 let rec len_of_num1 uu = one_nat;;
 
 let len0_num1 = ({len_of = len_of_num1} : num1 len0);;
+
+let one_integera : Big_int.big_int = (Big_int.big_int_of_int 1);;
+
+let one_integer = ({one = one_integera} : Big_int.big_int one);;
+
+let zero_integer = ({zero = Big_int.zero_big_int} : Big_int.big_int zero);;
+
+let zero_neq_one_integer =
+  ({one_zero_neq_one = one_integer; zero_zero_neq_one = zero_integer} :
+    Big_int.big_int zero_neq_one);;
 
 type storage_inst = SLOAD | SSTORE;;
 
@@ -114,11 +406,18 @@ type lllllogic = LLAnd | LLOr | LLNot;;
 type llllarith = LAPlus | LAMinus | LATimes | LADiv | LAMod | LAAnd | LAOr |
   LAXor | LANot | LAExp;;
 
-type llll = L4L_Str of char list | L4L_Nat of nat | L4I0 of inst |
-  L4I1 of inst * llll | L4I2 of inst * llll * llll | L4Seq of llll list |
+type llll = L4L_Str of char list | L4L_Int of int | L4I0 of inst |
+  L4I1 of inst * llll | L4I2 of inst * llll * llll |
+  L4I3 of inst * llll * llll * llll | L4I4 of inst * llll * llll * llll * llll |
+  L4In of inst * llll list | L4Seq of llll list |
   L4Arith of llllarith * llll list | L4Logic of lllllogic * llll list |
   L4Comp of llllcompare * llll * llll | L4When of llll * llll |
-  L4If of llll * llll * llll | L4While of llll * llll;;
+  L4Unless of llll * llll | L4If of llll * llll * llll |
+  L4For of llll * llll * llll * llll | L4Revert;;
+
+type ('a, 'b) tree = Leaf | Node of ('a, 'b) tree * 'a * 'b * ('a, 'b) tree;;
+
+type cmp_val = LT | EQ | GT;;
 
 type stree = STStr of char list | STStrs of stree list;;
 
@@ -129,16 +428,24 @@ type ('a, 'b, 'c, 'd, 'e, 'f, 'g) llt = La of 'a * inst | LLaba of 'b * nat |
   LJmpa of 'c * nat * nat | LJmpIa of 'd * nat * nat |
   LSeqa of 'e * ((nat * nat) * ('a, 'b, 'c, 'd, 'e, 'f, 'g) llt) list;;
 
+type 'a program_ext = Program_ext of (int -> inst option) * int * 'a;;
+
 type jump_resolve_result = JSuccess | JFail of nat list | JBump of nat list;;
 
-let rec eq _A a b = equal _A a b;;
+type 'a constant_ctx_ext =
+  Constant_ctx_ext of
+    unit program_ext * num1 bit0 bit1 bit0 bit0 bit0 bit0 bit0 word *
+      (num1 bit0 bit0 bit0 word list -> bool) * 'a;;
 
-let rec nat k = Nat (max ord_integer Big_int.zero_big_int (integer_of_int k));;
+let rec id x = (fun xa -> xa) x;;
 
-let rec plus_nat
-  m n = Nat (Big_int.add_big_int (integer_of_nat m) (integer_of_nat n));;
+let rec cmp (_A1, _A2)
+  x y = (if less _A2.order_linorder.preorder_order.ord_preorder x y then LT
+          else (if eq _A1 x y then EQ else GT));;
 
-let rec suc n = plus_nat n one_nat;;
+let rec nat = function Pos k -> nat_of_num k
+              | Zero_int -> Zero_nat
+              | Neg k -> Zero_nat;;
 
 let rec comp f g = (fun x -> f (g x));;
 
@@ -157,19 +464,1002 @@ let rec uint _A (Word x) = x;;
 
 let rec unat _A w = nat (uint _A w);;
 
-let rec char_of_nat
-  x = comp (fun a -> Char.chr (Big_int.int_of_big_int a)) integer_of_nat x;;
+let rec ht = function Leaf -> Zero_nat
+             | Node (l, a, h, r) -> h;;
 
-let apos : char = char_of_nat (nat_of_integer (Big_int.big_int_of_int 39));;
+let rec bit_cut_integer
+  k = (if Big_int.eq_big_int k Big_int.zero_big_int
+        then (Big_int.zero_big_int, false)
+        else (let (r, s) =
+                Big_int.quomod_big_int (Big_int.abs_big_int k)
+                  (Big_int.abs_big_int (Big_int.big_int_of_int 2))
+                in
+               ((if Big_int.lt_big_int Big_int.zero_big_int k then r
+                  else Big_int.sub_big_int (Big_int.minus_big_int r) s),
+                 Big_int.eq_big_int s (Big_int.big_int_of_int 1))));;
 
-let zero_nat : nat = Nat Big_int.zero_big_int;;
+let rec char_of_integer
+  k = (let (q0, b0) = bit_cut_integer k in
+       let (q1, b1) = bit_cut_integer q0 in
+       let (q2, b2) = bit_cut_integer q1 in
+       let (q3, b3) = bit_cut_integer q2 in
+       let (q4, b4) = bit_cut_integer q3 in
+       let (q5, b5) = bit_cut_integer q4 in
+       let (q6, b6) = bit_cut_integer q5 in
+       let a = bit_cut_integer q6 in
+       let (_, aa) = a in
+        Chara (b0, b1, b2, b3, b4, b5, b6, aa));;
 
-let rec gen_length n x1 = match n, x1 with n, x :: xs -> gen_length (suc n) xs
+let apos : char = char_of_integer (Big_int.big_int_of_int 39);;
+
+let rec gen_length n x1 = match n, x1 with n, x :: xs -> gen_length (Suc n) xs
                      | n, [] -> n;;
 
-let rec size_list x = gen_length zero_nat x;;
+let rec size_list x = gen_length Zero_nat x;;
 
-let rec int_of_nat n = Int_of_integer (integer_of_nat n);;
+let rec of_nat_aux _A inc x1 i = match inc, x1, i with inc, Zero_nat, i -> i
+                        | inc, Suc n, i -> of_nat_aux _A inc n (inc i);;
+
+let rec of_nat _A
+  n = of_nat_aux _A
+        (fun i ->
+          plus _A.semiring_numeral_semiring_1.numeral_semiring_numeral.semigroup_add_numeral.plus_semigroup_add
+            i (one _A.semiring_numeral_semiring_1.numeral_semiring_numeral.one_numeral))
+        n (zero _A.semiring_0_semiring_1.mult_zero_semiring_0.zero_mult_zero);;
+
+let rec divmod_step_int
+  l (q, r) =
+    (if less_eq_int (Pos l) r
+      then (plus_inta (times_inta (Pos (Bit0 One)) q) one_inta,
+             minus_int r (Pos l))
+      else (times_inta (Pos (Bit0 One)) q, r));;
+
+let rec divmod_int
+  x0 x1 = match x0, x1 with
+    Bit1 m, Bit1 n ->
+      (if less_num m n then (Zero_int, Pos (Bit1 m))
+        else divmod_step_int (Bit1 n) (divmod_int (Bit1 m) (Bit0 (Bit1 n))))
+    | Bit0 m, Bit1 n ->
+        (if less_eq_num m n then (Zero_int, Pos (Bit0 m))
+          else divmod_step_int (Bit1 n) (divmod_int (Bit0 m) (Bit0 (Bit1 n))))
+    | Bit1 m, Bit0 n ->
+        (let (q, r) = divmod_int m n in
+          (q, plus_inta (times_inta (Pos (Bit0 One)) r) one_inta))
+    | Bit0 m, Bit0 n ->
+        (let (q, r) = divmod_int m n in (q, times_inta (Pos (Bit0 One)) r))
+    | One, Bit1 n -> (Zero_int, Pos One)
+    | One, Bit0 n -> (Zero_int, Pos One)
+    | Bit1 m, One -> (Pos (Bit1 m), Zero_int)
+    | Bit0 m, One -> (Pos (Bit0 m), Zero_int)
+    | One, One -> (Pos One, Zero_int);;
+
+let rec snd (x1, x2) = x2;;
+
+let rec adjust_mod
+  l r = (if equal_inta r Zero_int then Zero_int else minus_int l r);;
+
+let rec modulo_int
+  k ka = match k, ka with Neg m, Neg n -> uminus_int (snd (divmod_int m n))
+    | Pos m, Neg n -> uminus_int (adjust_mod (Pos n) (snd (divmod_int m n)))
+    | Neg m, Pos n -> adjust_mod (Pos n) (snd (divmod_int m n))
+    | Pos m, Pos n -> snd (divmod_int m n)
+    | k, Neg One -> Zero_int
+    | k, Pos One -> Zero_int
+    | Zero_int, k -> Zero_int
+    | k, Zero_int -> k;;
+
+let rec power _A a x1 = match a, x1 with a, Zero_nat -> one _A.one_power
+                   | a, Suc n -> times _A.times_power a (power _A a n);;
+
+let rec word_of_int _A
+  k = Word (modulo_int k (power power_int (Pos (Bit0 One)) (len_of _A Type)));;
+
+let rec storage_inst_code
+  = function
+    SLOAD ->
+      word_of_int (len0_bit0 (len0_bit0 (len0_bit0 len0_num1)))
+        (Pos (Bit0 (Bit0 (Bit1 (Bit0 (Bit1 (Bit0 One)))))))
+    | SSTORE ->
+        word_of_int (len0_bit0 (len0_bit0 (len0_bit0 len0_num1)))
+          (Pos (Bit1 (Bit0 (Bit1 (Bit0 (Bit1 (Bit0 One)))))));;
+
+let rec sarith_inst_code
+  = function
+    SDIV ->
+      word_of_int (len0_bit0 (len0_bit0 (len0_bit0 len0_num1)))
+        (Pos (Bit1 (Bit0 One)))
+    | SMOD ->
+        word_of_int (len0_bit0 (len0_bit0 (len0_bit0 len0_num1)))
+          (Pos (Bit1 (Bit1 One)))
+    | SGT ->
+        word_of_int (len0_bit0 (len0_bit0 (len0_bit0 len0_num1)))
+          (Pos (Bit1 (Bit1 (Bit0 (Bit0 One)))))
+    | SLT ->
+        word_of_int (len0_bit0 (len0_bit0 (len0_bit0 len0_num1)))
+          (Pos (Bit0 (Bit1 (Bit0 (Bit0 One)))))
+    | SIGNEXTEND ->
+        word_of_int (len0_bit0 (len0_bit0 (len0_bit0 len0_num1)))
+          (Pos (Bit1 (Bit1 (Bit0 One))));;
+
+let rec memory_inst_code
+  = function
+    MLOAD ->
+      word_of_int (len0_bit0 (len0_bit0 (len0_bit0 len0_num1)))
+        (Pos (Bit1 (Bit0 (Bit0 (Bit0 (Bit1 (Bit0 One)))))))
+    | MSTORE ->
+        word_of_int (len0_bit0 (len0_bit0 (len0_bit0 len0_num1)))
+          (Pos (Bit0 (Bit1 (Bit0 (Bit0 (Bit1 (Bit0 One)))))))
+    | MSTORE8 ->
+        word_of_int (len0_bit0 (len0_bit0 (len0_bit0 len0_num1)))
+          (Pos (Bit1 (Bit1 (Bit0 (Bit0 (Bit1 (Bit0 One)))))))
+    | CALLDATACOPY ->
+        word_of_int (len0_bit0 (len0_bit0 (len0_bit0 len0_num1)))
+          (Pos (Bit1 (Bit1 (Bit1 (Bit0 (Bit1 One))))))
+    | CODECOPY ->
+        word_of_int (len0_bit0 (len0_bit0 (len0_bit0 len0_num1)))
+          (Pos (Bit1 (Bit0 (Bit0 (Bit1 (Bit1 One))))))
+    | EXTCODECOPY ->
+        word_of_int (len0_bit0 (len0_bit0 (len0_bit0 len0_num1)))
+          (Pos (Bit0 (Bit0 (Bit1 (Bit1 (Bit1 One))))))
+    | MSIZE ->
+        word_of_int (len0_bit0 (len0_bit0 (len0_bit0 len0_num1)))
+          (Pos (Bit1 (Bit0 (Bit0 (Bit1 (Bit1 (Bit0 One)))))));;
+
+let rec plus_word _A a b = word_of_int _A (plus_inta (uint _A a) (uint _A b));;
+
+let rec word8FromNat
+  i = word_of_int (len0_bit0 (len0_bit0 (len0_bit0 len0_num1)))
+        (of_nat semiring_1_int i);;
+
+let rec byteFromNat x = word8FromNat x;;
+
+let rec stack_inst_code
+  = function
+    POP ->
+      [word_of_int (len0_bit0 (len0_bit0 (len0_bit0 len0_num1)))
+         (Pos (Bit0 (Bit0 (Bit0 (Bit0 (Bit1 (Bit0 One)))))))]
+    | PUSH_N lst ->
+        (if less_nat (size_list lst) one_nat
+          then [word_of_int (len0_bit0 (len0_bit0 (len0_bit0 len0_num1)))
+                  (Pos (Bit0 (Bit0 (Bit0 (Bit0 (Bit0 (Bit1 One)))))));
+                 word_of_int (len0_bit0 (len0_bit0 (len0_bit0 len0_num1)))
+                   Zero_int]
+          else (if less_nat (nat_of_num (Bit0 (Bit0 (Bit0 (Bit0 (Bit0 One))))))
+                     (size_list lst)
+                 then [word_of_int (len0_bit0 (len0_bit0 (len0_bit0 len0_num1)))
+                         (Pos (Bit0 (Bit0 (Bit0 (Bit0 (Bit0 (Bit1 One)))))));
+                        word_of_int
+                          (len0_bit0 (len0_bit0 (len0_bit0 len0_num1)))
+                          Zero_int]
+                 else [plus_word (len0_bit0 (len0_bit0 (len0_bit0 len0_num1)))
+                         (byteFromNat (size_list lst))
+                         (word_of_int
+                           (len0_bit0 (len0_bit0 (len0_bit0 len0_num1)))
+                           (Pos (Bit1 (Bit1
+(Bit1 (Bit1 (Bit1 (Bit0 One))))))))] @
+                        lst))
+    | CALLDATALOAD ->
+        [word_of_int (len0_bit0 (len0_bit0 (len0_bit0 len0_num1)))
+           (Pos (Bit1 (Bit0 (Bit1 (Bit0 (Bit1 One))))))];;
+
+let rec arith_inst_code
+  = function
+    ADD -> word_of_int (len0_bit0 (len0_bit0 (len0_bit0 len0_num1))) one_inta
+    | MUL ->
+        word_of_int (len0_bit0 (len0_bit0 (len0_bit0 len0_num1)))
+          (Pos (Bit0 One))
+    | SUB ->
+        word_of_int (len0_bit0 (len0_bit0 (len0_bit0 len0_num1)))
+          (Pos (Bit1 One))
+    | DIV ->
+        word_of_int (len0_bit0 (len0_bit0 (len0_bit0 len0_num1)))
+          (Pos (Bit0 (Bit0 One)))
+    | MOD ->
+        word_of_int (len0_bit0 (len0_bit0 (len0_bit0 len0_num1)))
+          (Pos (Bit0 (Bit1 One)))
+    | ADDMOD ->
+        word_of_int (len0_bit0 (len0_bit0 (len0_bit0 len0_num1)))
+          (Pos (Bit0 (Bit0 (Bit0 One))))
+    | MULMOD ->
+        word_of_int (len0_bit0 (len0_bit0 (len0_bit0 len0_num1)))
+          (Pos (Bit1 (Bit0 (Bit0 One))))
+    | EXP ->
+        word_of_int (len0_bit0 (len0_bit0 (len0_bit0 len0_num1)))
+          (Pos (Bit0 (Bit1 (Bit0 One))))
+    | Inst_GT ->
+        word_of_int (len0_bit0 (len0_bit0 (len0_bit0 len0_num1)))
+          (Pos (Bit1 (Bit0 (Bit0 (Bit0 One)))))
+    | Inst_LT ->
+        word_of_int (len0_bit0 (len0_bit0 (len0_bit0 len0_num1)))
+          (Pos (Bit0 (Bit0 (Bit0 (Bit0 One)))))
+    | Inst_EQ ->
+        word_of_int (len0_bit0 (len0_bit0 (len0_bit0 len0_num1)))
+          (Pos (Bit0 (Bit0 (Bit1 (Bit0 One)))))
+    | ISZERO ->
+        word_of_int (len0_bit0 (len0_bit0 (len0_bit0 len0_num1)))
+          (Pos (Bit1 (Bit0 (Bit1 (Bit0 One)))))
+    | SHA3 ->
+        word_of_int (len0_bit0 (len0_bit0 (len0_bit0 len0_num1)))
+          (Pos (Bit0 (Bit0 (Bit0 (Bit0 (Bit0 One))))));;
+
+let rec swap_inst_code
+  m = plus_word (len0_bit0 (len0_bit0 (len0_bit0 len0_num1)))
+        (word_of_int (len0_bit0 (len0_bit0 (len0_bit0 len0_num1)))
+          (uint (len0_bit0 (len0_bit0 len0_num1)) m))
+        (word_of_int (len0_bit0 (len0_bit0 (len0_bit0 len0_num1)))
+          (Pos (Bit0 (Bit0 (Bit0 (Bit0 (Bit1 (Bit0 (Bit0 One)))))))));;
+
+let rec misc_inst_code
+  = function
+    STOP -> word_of_int (len0_bit0 (len0_bit0 (len0_bit0 len0_num1))) Zero_int
+    | CREATE ->
+        word_of_int (len0_bit0 (len0_bit0 (len0_bit0 len0_num1)))
+          (Pos (Bit0 (Bit0 (Bit0 (Bit0 (Bit1 (Bit1 (Bit1 One))))))))
+    | CALL ->
+        word_of_int (len0_bit0 (len0_bit0 (len0_bit0 len0_num1)))
+          (Pos (Bit1 (Bit0 (Bit0 (Bit0 (Bit1 (Bit1 (Bit1 One))))))))
+    | CALLCODE ->
+        word_of_int (len0_bit0 (len0_bit0 (len0_bit0 len0_num1)))
+          (Pos (Bit0 (Bit1 (Bit0 (Bit0 (Bit1 (Bit1 (Bit1 One))))))))
+    | RETURN ->
+        word_of_int (len0_bit0 (len0_bit0 (len0_bit0 len0_num1)))
+          (Pos (Bit1 (Bit1 (Bit0 (Bit0 (Bit1 (Bit1 (Bit1 One))))))))
+    | DELEGATECALL ->
+        word_of_int (len0_bit0 (len0_bit0 (len0_bit0 len0_num1)))
+          (Pos (Bit0 (Bit0 (Bit1 (Bit0 (Bit1 (Bit1 (Bit1 One))))))))
+    | SUICIDE ->
+        word_of_int (len0_bit0 (len0_bit0 (len0_bit0 len0_num1)))
+          (Pos (Bit1 (Bit1 (Bit1 (Bit1 (Bit1 (Bit1 (Bit1 One))))))));;
+
+let rec info_inst_code
+  = function
+    ADDRESS ->
+      word_of_int (len0_bit0 (len0_bit0 (len0_bit0 len0_num1)))
+        (Pos (Bit0 (Bit0 (Bit0 (Bit0 (Bit1 One))))))
+    | BALANCE ->
+        word_of_int (len0_bit0 (len0_bit0 (len0_bit0 len0_num1)))
+          (Pos (Bit1 (Bit0 (Bit0 (Bit0 (Bit1 One))))))
+    | ORIGIN ->
+        word_of_int (len0_bit0 (len0_bit0 (len0_bit0 len0_num1)))
+          (Pos (Bit0 (Bit1 (Bit0 (Bit0 (Bit1 One))))))
+    | CALLVALUE ->
+        word_of_int (len0_bit0 (len0_bit0 (len0_bit0 len0_num1)))
+          (Pos (Bit0 (Bit0 (Bit1 (Bit0 (Bit1 One))))))
+    | CALLDATASIZE ->
+        word_of_int (len0_bit0 (len0_bit0 (len0_bit0 len0_num1)))
+          (Pos (Bit0 (Bit1 (Bit1 (Bit0 (Bit1 One))))))
+    | CALLER ->
+        word_of_int (len0_bit0 (len0_bit0 (len0_bit0 len0_num1)))
+          (Pos (Bit1 (Bit1 (Bit0 (Bit0 (Bit1 One))))))
+    | CODESIZE ->
+        word_of_int (len0_bit0 (len0_bit0 (len0_bit0 len0_num1)))
+          (Pos (Bit0 (Bit0 (Bit0 (Bit1 (Bit1 One))))))
+    | GASPRICE ->
+        word_of_int (len0_bit0 (len0_bit0 (len0_bit0 len0_num1)))
+          (Pos (Bit0 (Bit1 (Bit0 (Bit1 (Bit1 One))))))
+    | EXTCODESIZE ->
+        word_of_int (len0_bit0 (len0_bit0 (len0_bit0 len0_num1)))
+          (Pos (Bit1 (Bit1 (Bit0 (Bit1 (Bit1 One))))))
+    | BLOCKHASH ->
+        word_of_int (len0_bit0 (len0_bit0 (len0_bit0 len0_num1)))
+          (Pos (Bit0 (Bit0 (Bit0 (Bit0 (Bit0 (Bit0 One)))))))
+    | COINBASE ->
+        word_of_int (len0_bit0 (len0_bit0 (len0_bit0 len0_num1)))
+          (Pos (Bit1 (Bit0 (Bit0 (Bit0 (Bit0 (Bit0 One)))))))
+    | TIMESTAMP ->
+        word_of_int (len0_bit0 (len0_bit0 (len0_bit0 len0_num1)))
+          (Pos (Bit0 (Bit1 (Bit0 (Bit0 (Bit0 (Bit0 One)))))))
+    | NUMBER ->
+        word_of_int (len0_bit0 (len0_bit0 (len0_bit0 len0_num1)))
+          (Pos (Bit1 (Bit1 (Bit0 (Bit0 (Bit0 (Bit0 One)))))))
+    | DIFFICULTY ->
+        word_of_int (len0_bit0 (len0_bit0 (len0_bit0 len0_num1)))
+          (Pos (Bit0 (Bit0 (Bit1 (Bit0 (Bit0 (Bit0 One)))))))
+    | GASLIMIT ->
+        word_of_int (len0_bit0 (len0_bit0 (len0_bit0 len0_num1)))
+          (Pos (Bit1 (Bit0 (Bit1 (Bit0 (Bit0 (Bit0 One)))))))
+    | GAS ->
+        word_of_int (len0_bit0 (len0_bit0 (len0_bit0 len0_num1)))
+          (Pos (Bit0 (Bit1 (Bit0 (Bit1 (Bit1 (Bit0 One)))))));;
+
+let rec bits_inst_code
+  = function
+    Inst_AND ->
+      word_of_int (len0_bit0 (len0_bit0 (len0_bit0 len0_num1)))
+        (Pos (Bit0 (Bit1 (Bit1 (Bit0 One)))))
+    | Inst_OR ->
+        word_of_int (len0_bit0 (len0_bit0 (len0_bit0 len0_num1)))
+          (Pos (Bit1 (Bit1 (Bit1 (Bit0 One)))))
+    | Inst_XOR ->
+        word_of_int (len0_bit0 (len0_bit0 (len0_bit0 len0_num1)))
+          (Pos (Bit0 (Bit0 (Bit0 (Bit1 One)))))
+    | Inst_NOT ->
+        word_of_int (len0_bit0 (len0_bit0 (len0_bit0 len0_num1)))
+          (Pos (Bit1 (Bit0 (Bit0 (Bit1 One)))))
+    | BYTE ->
+        word_of_int (len0_bit0 (len0_bit0 (len0_bit0 len0_num1)))
+          (Pos (Bit0 (Bit1 (Bit0 (Bit1 One)))));;
+
+let rec log_inst_code
+  = function
+    LOG0 ->
+      word_of_int (len0_bit0 (len0_bit0 (len0_bit0 len0_num1)))
+        (Pos (Bit0 (Bit0 (Bit0 (Bit0 (Bit0 (Bit1 (Bit0 One))))))))
+    | LOG1 ->
+        word_of_int (len0_bit0 (len0_bit0 (len0_bit0 len0_num1)))
+          (Pos (Bit1 (Bit0 (Bit0 (Bit0 (Bit0 (Bit1 (Bit0 One))))))))
+    | LOG2 ->
+        word_of_int (len0_bit0 (len0_bit0 (len0_bit0 len0_num1)))
+          (Pos (Bit0 (Bit1 (Bit0 (Bit0 (Bit0 (Bit1 (Bit0 One))))))))
+    | LOG3 ->
+        word_of_int (len0_bit0 (len0_bit0 (len0_bit0 len0_num1)))
+          (Pos (Bit1 (Bit1 (Bit0 (Bit0 (Bit0 (Bit1 (Bit0 One))))))))
+    | LOG4 ->
+        word_of_int (len0_bit0 (len0_bit0 (len0_bit0 len0_num1)))
+          (Pos (Bit0 (Bit0 (Bit1 (Bit0 (Bit0 (Bit1 (Bit0 One))))))));;
+
+let rec dup_inst_code
+  m = plus_word (len0_bit0 (len0_bit0 (len0_bit0 len0_num1)))
+        (word_of_int (len0_bit0 (len0_bit0 (len0_bit0 len0_num1)))
+          (uint (len0_bit0 (len0_bit0 len0_num1)) m))
+        (word_of_int (len0_bit0 (len0_bit0 (len0_bit0 len0_num1)))
+          (Pos (Bit0 (Bit0 (Bit0 (Bit0 (Bit0 (Bit0 (Bit0 One)))))))));;
+
+let rec pc_inst_code
+  = function
+    JUMP ->
+      word_of_int (len0_bit0 (len0_bit0 (len0_bit0 len0_num1)))
+        (Pos (Bit0 (Bit1 (Bit1 (Bit0 (Bit1 (Bit0 One)))))))
+    | JUMPI ->
+        word_of_int (len0_bit0 (len0_bit0 (len0_bit0 len0_num1)))
+          (Pos (Bit1 (Bit1 (Bit1 (Bit0 (Bit1 (Bit0 One)))))))
+    | PC -> word_of_int (len0_bit0 (len0_bit0 (len0_bit0 len0_num1)))
+              (Pos (Bit0 (Bit0 (Bit0 (Bit1 (Bit1 (Bit0 One)))))))
+    | JUMPDEST ->
+        word_of_int (len0_bit0 (len0_bit0 (len0_bit0 len0_num1)))
+          (Pos (Bit1 (Bit1 (Bit0 (Bit1 (Bit1 (Bit0 One)))))));;
+
+let rec inst_code = function Unknown byte -> [byte]
+                    | Bits b -> [bits_inst_code b]
+                    | Sarith s -> [sarith_inst_code s]
+                    | Arith a -> [arith_inst_code a]
+                    | Info i -> [info_inst_code i]
+                    | Dup d -> [dup_inst_code d]
+                    | Memory m -> [memory_inst_code m]
+                    | Storage s -> [storage_inst_code s]
+                    | Pc p -> [pc_inst_code p]
+                    | Stack s -> stack_inst_code s
+                    | Swap s -> [swap_inst_code s]
+                    | Log l -> [log_inst_code l]
+                    | Misc m -> [misc_inst_code m];;
+
+let rec inst_size i = of_nat semiring_1_int (size_list (inst_code i));;
+
+let rec ilsz = function [] -> Zero_nat
+               | h :: t -> plus_nat (nat (inst_size h)) (ilsz t);;
+
+let rec map f x1 = match f, x1 with f, [] -> []
+              | f, x21 :: x22 -> f x21 :: map f x22;;
+
+let rec member _A x0 y = match x0, y with [], y -> false
+                    | x :: xs, y -> eq _A x y || member _A xs y;;
+
+let rec isWs
+  x = member equal_char
+        (map char_of_integer
+          [(Big_int.big_int_of_int 9); (Big_int.big_int_of_int 10);
+            (Big_int.big_int_of_int 11); (Big_int.big_int_of_int 12);
+            (Big_int.big_int_of_int 13); (Big_int.big_int_of_int 32)])
+        x;;
+
+let rec foldl f a x2 = match f, a, x2 with f, a, [] -> a
+                | f, a, x :: xs -> foldl f (f a x) xs;;
+
+let rec foldr f x1 = match f, x1 with f, [] -> id
+                | f, x :: xs -> comp (f x) (foldr f xs);;
+
+let rec map_option f x1 = match f, x1 with f, None -> None
+                     | f, Some x2 -> Some (f x2);;
+
+let rec those
+  = function [] -> Some []
+    | x :: xs ->
+        (match x with None -> None
+          | Some y -> map_option (fun a -> y :: a) (those xs));;
+
+let rec map_of _A
+  x0 k = match x0, k with
+    (l, v) :: ps, k -> (if eq _A l k then Some v else map_of _A ps k)
+    | [], k -> None;;
+
+let quote : char = char_of_integer (Big_int.big_int_of_int 34);;
+
+let rec concat xss = foldr (fun a b -> a @ b) xss [];;
+
+let rec max _A a b = (if less_eq _A a b then b else a);;
+
+let rec node
+  l a r = Node (l, a, plus_nat (max ord_nat (ht l) (ht r)) one_nat, r);;
+
+let rec balL
+  l a r =
+    (if equal_nata (ht l) (plus_nat (ht r) (nat_of_num (Bit0 One)))
+      then (let Node (bl, b, _, br) = l in
+             (if less_nat (ht bl) (ht br)
+               then (let Node (cl, c, _, cr) = br in
+                      node (node bl b cl) c (node cr a r))
+               else node bl b (node br a r)))
+      else node l a r);;
+
+let rec balR
+  l a r =
+    (if equal_nata (ht r) (plus_nat (ht l) (nat_of_num (Bit0 One)))
+      then (let Node (bl, b, _, br) = r in
+             (if less_nat (ht br) (ht bl)
+               then (let Node (cl, c, _, cr) = bl in
+                      node (node l a cl) c (node cr b br))
+               else node (node l a bl) b br))
+      else node l a r);;
+
+let rec lookupS
+  x0 uu = match x0, uu with [], uu -> None
+    | (ah, bh) :: t, a ->
+        (if equal_lista equal_char a ah then Some bh else lookupS t a);;
+
+let newline : char = char_of_integer (Big_int.big_int_of_int 10);;
+
+let rec update (_A1, _A2)
+  x y xa2 = match x, y, xa2 with
+    x, y, Leaf -> Node (Leaf, (x, y), one_nat, Leaf)
+    | x, y, Node (l, (a, b), h, r) ->
+        (match cmp (_A1, _A2) x a
+          with LT -> balL (update (_A1, _A2) x y l) (a, b) r
+          | EQ -> Node (l, (x, y), h, r)
+          | GT -> balR l (a, b) (update (_A1, _A2) x y r));;
+
+let rec mkConsts
+  x0 x1 = match x0, x1 with [], [] -> Some []
+    | sh :: st, lh :: lt ->
+        (match mkConsts st lt with None -> None
+          | Some ft -> Some ((sh, (fun _ -> Some lh)) :: ft))
+    | v :: va, [] -> None
+    | [], v :: va -> None;;
+
+let hex_parse_table : (char * int) list
+  = [(Chara (false, false, false, false, true, true, false, false), Zero_int);
+      (Chara (true, false, false, false, true, true, false, false), one_inta);
+      (Chara (false, true, false, false, true, true, false, false),
+        Pos (Bit0 One));
+      (Chara (true, true, false, false, true, true, false, false),
+        Pos (Bit1 One));
+      (Chara (false, false, true, false, true, true, false, false),
+        Pos (Bit0 (Bit0 One)));
+      (Chara (true, false, true, false, true, true, false, false),
+        Pos (Bit1 (Bit0 One)));
+      (Chara (false, true, true, false, true, true, false, false),
+        Pos (Bit0 (Bit1 One)));
+      (Chara (true, true, true, false, true, true, false, false),
+        Pos (Bit1 (Bit1 One)));
+      (Chara (false, false, false, true, true, true, false, false),
+        Pos (Bit0 (Bit0 (Bit0 One))));
+      (Chara (true, false, false, true, true, true, false, false),
+        Pos (Bit1 (Bit0 (Bit0 One))));
+      (Chara (true, false, false, false, false, false, true, false),
+        Pos (Bit0 (Bit1 (Bit0 One))));
+      (Chara (true, false, false, false, false, true, true, false),
+        Pos (Bit0 (Bit1 (Bit0 One))));
+      (Chara (false, true, false, false, false, false, true, false),
+        Pos (Bit1 (Bit1 (Bit0 One))));
+      (Chara (false, true, false, false, false, true, true, false),
+        Pos (Bit1 (Bit1 (Bit0 One))));
+      (Chara (true, true, false, false, false, false, true, false),
+        Pos (Bit0 (Bit0 (Bit1 One))));
+      (Chara (true, true, false, false, false, true, true, false),
+        Pos (Bit0 (Bit0 (Bit1 One))));
+      (Chara (false, false, true, false, false, false, true, false),
+        Pos (Bit1 (Bit0 (Bit1 One))));
+      (Chara (false, false, true, false, false, true, true, false),
+        Pos (Bit1 (Bit0 (Bit1 One))));
+      (Chara (true, false, true, false, false, false, true, false),
+        Pos (Bit0 (Bit1 (Bit1 One))));
+      (Chara (true, false, true, false, false, true, true, false),
+        Pos (Bit0 (Bit1 (Bit1 One))));
+      (Chara (false, true, true, false, false, false, true, false),
+        Pos (Bit1 (Bit1 (Bit1 One))));
+      (Chara (false, true, true, false, false, true, true, false),
+        Pos (Bit1 (Bit1 (Bit1 One))))];;
+
+let rec parseHexNumeral
+  x0 s f r = match x0, s, f, r with [], s, f, r -> f []
+    | h :: t, s, f, r ->
+        (match map_of equal_char hex_parse_table h with None -> f (h :: t)
+          | Some n -> s n t);;
+
+let rec parseHexSub
+  i x1 su fa r = match i, x1, su, fa, r with i, [], su, fa, r -> su i []
+    | i, h :: t, su, fa, r ->
+        parseHexNumeral (h :: t)
+          (fun n l ->
+            parseHexSub
+              (plus_inta (times_inta (Pos (Bit0 (Bit0 (Bit0 (Bit0 One))))) i) n)
+              l su fa r)
+          (su i) r;;
+
+let rec parseHex
+  x0 su fa r = match x0, su, fa, r with
+    h0 :: hx :: h :: t, su, fa, r ->
+      (if equal_chara h0
+            (Chara (false, false, false, false, true, true, false, false)) &&
+            equal_chara hx
+              (Chara (false, false, false, true, true, true, true, false))
+        then parseHexNumeral (h :: t) (fun n l -> parseHexSub n l su fa r) fa r
+        else fa (h0 :: hx :: h :: t))
+    | [], su, fa, r -> fa []
+    | [v], su, fa, r -> fa [v]
+    | [v; vb], su, fa, r -> fa [v; vb];;
+
+let rec is_digit_char
+  c = equal_chara c
+        (Chara (false, false, false, false, true, true, false, false)) ||
+        (equal_chara c
+           (Chara (true, false, true, false, true, true, false, false)) ||
+          (equal_chara c
+             (Chara (true, false, false, false, true, true, false, false)) ||
+            (equal_chara c
+               (Chara (false, true, true, false, true, true, false, false)) ||
+              (equal_chara c
+                 (Chara
+                   (false, true, false, false, true, true, false, false)) ||
+                (equal_chara c
+                   (Chara
+                     (true, true, true, false, true, true, false, false)) ||
+                  (equal_chara c
+                     (Chara
+                       (true, true, false, false, true, true, false, false)) ||
+                    (equal_chara c
+                       (Chara
+                         (false, false, false, true, true, true, false,
+                           false)) ||
+                      (equal_chara c
+                         (Chara
+                           (false, false, true, false, true, true, false,
+                             false)) ||
+                        equal_chara c
+                          (Chara
+                            (true, false, false, true, true, true, false,
+                              false))))))))));;
+
+let rec char_to_digit
+  c = (if equal_chara c
+            (Chara (false, false, false, false, true, true, false, false))
+        then Zero_nat
+        else (if equal_chara c
+                   (Chara (true, false, false, false, true, true, false, false))
+               then one_nat
+               else (if equal_chara c
+                          (Chara
+                            (false, true, false, false, true, true, false,
+                              false))
+                      then nat_of_num (Bit0 One)
+                      else (if equal_chara c
+                                 (Chara
+                                   (true, true, false, false, true, true, false,
+                                     false))
+                             then nat_of_num (Bit1 One)
+                             else (if equal_chara c
+(Chara (false, false, true, false, true, true, false, false))
+                                    then nat_of_num (Bit0 (Bit0 One))
+                                    else (if equal_chara c
+       (Chara (true, false, true, false, true, true, false, false))
+   then nat_of_num (Bit1 (Bit0 One))
+   else (if equal_chara c
+              (Chara (false, true, true, false, true, true, false, false))
+          then nat_of_num (Bit0 (Bit1 One))
+          else (if equal_chara c
+                     (Chara (true, true, true, false, true, true, false, false))
+                 then nat_of_num (Bit1 (Bit1 One))
+                 else (if equal_chara c
+                            (Chara
+                              (false, false, false, true, true, true, false,
+                                false))
+                        then nat_of_num (Bit0 (Bit0 (Bit0 One)))
+                        else (if equal_chara c
+                                   (Chara
+                                     (true, false, false, true, true, true,
+                                       false, false))
+                               then nat_of_num (Bit1 (Bit0 (Bit0 One)))
+                               else nat_of_num
+                                      (Bit0 (Bit1 (Bit0 One)))))))))))));;
+
+let rec parseNumeral
+  x0 s f r = match x0, s, f, r with [], s, f, r -> f []
+    | h :: t, s, f, r ->
+        (if is_digit_char h then s (of_nat semiring_1_int (char_to_digit h)) t
+          else f (h :: t));;
+
+let rec parseIntSub
+  i x1 su fa r = match i, x1, su, fa, r with i, [], su, fa, r -> su i []
+    | i, h :: t, su, fa, r ->
+        parseNumeral (h :: t)
+          (fun n l ->
+            parseIntSub
+              (plus_inta (times_inta (Pos (Bit0 (Bit1 (Bit0 One)))) i) n) l su
+              fa r)
+          (su i) r;;
+
+let rec parseInt
+  x0 su fa r = match x0, su, fa, r with [], su, fa, r -> fa []
+    | h :: t, su, fa, r ->
+        parseNumeral (h :: t) (fun n l -> parseIntSub n l su fa r) fa r;;
+
+let rec lookup (_A1, _A2)
+  xa0 x = match xa0, x with Leaf, x -> None
+    | Node (l, (a, b), uu, r), x ->
+        (match cmp (_A1, _A2) x a with LT -> lookup (_A1, _A2) l x
+          | EQ -> Some b | GT -> lookup (_A1, _A2) r x);;
+
+let rec of_bool _A = function true -> one _A.one_zero_neq_one
+                     | false -> zero _A.zero_zero_neq_one;;
+
+let rec integer_of_char
+  (Chara (b0, b1, b2, b3, b4, b5, b6, b7)) =
+    Big_int.add_big_int
+      (Big_int.mult_big_int
+        (Big_int.add_big_int
+          (Big_int.mult_big_int
+            (Big_int.add_big_int
+              (Big_int.mult_big_int
+                (Big_int.add_big_int
+                  (Big_int.mult_big_int
+                    (Big_int.add_big_int
+                      (Big_int.mult_big_int
+                        (Big_int.add_big_int
+                          (Big_int.mult_big_int
+                            (Big_int.add_big_int
+                              (Big_int.mult_big_int
+                                (of_bool zero_neq_one_integer b7)
+                                (Big_int.big_int_of_int 2))
+                              (of_bool zero_neq_one_integer b6))
+                            (Big_int.big_int_of_int 2))
+                          (of_bool zero_neq_one_integer b5))
+                        (Big_int.big_int_of_int 2))
+                      (of_bool zero_neq_one_integer b4))
+                    (Big_int.big_int_of_int 2))
+                  (of_bool zero_neq_one_integer b3))
+                (Big_int.big_int_of_int 2))
+              (of_bool zero_neq_one_integer b2))
+            (Big_int.big_int_of_int 2))
+          (of_bool zero_neq_one_integer b1))
+        (Big_int.big_int_of_int 2))
+      (of_bool zero_neq_one_integer b0);;
+
+let rec implode
+  cs = (let ks = (map integer_of_char
+                   cs) in let res = Bytes.create (List.length ks) in let rec imp i = function | [] -> res | k :: ks ->
+      let l = Big_int.int_of_big_int k in if 0 <= l && l < 128 then Bytes.set res i (Char.chr l) else failwith "Non-ASCII character in literal"; imp (i + 1) ks in imp 0 ks);;
+
+let rec fst (x1, x2) = x1;;
+
+let rec adjust_div
+  (q, r) =
+    plus_inta q (of_bool zero_neq_one_int (not (equal_inta r Zero_int)));;
+
+let rec divide_int
+  k ka = match k, ka with Neg m, Neg n -> fst (divmod_int m n)
+    | Pos m, Neg n -> uminus_int (adjust_div (divmod_int m n))
+    | Neg m, Pos n -> uminus_int (adjust_div (divmod_int m n))
+    | Pos m, Pos n -> fst (divmod_int m n)
+    | k, Neg One -> uminus_int k
+    | k, Pos One -> k
+    | Zero_int, k -> Zero_int
+    | k, Zero_int -> Zero_int;;
+
+let rec log256floor
+  x = (if less_eq_int x
+            (Pos (Bit1 (Bit1 (Bit1 (Bit1 (Bit1 (Bit1 (Bit1 One))))))))
+        then Zero_int
+        else plus_inta one_inta
+               (log256floor
+                 (divide_int x
+                   (Pos (Bit0 (Bit0 (Bit0 (Bit0
+    (Bit0 (Bit0 (Bit0 (Bit0 One))))))))))));;
+
+let rec run_parse
+  p donea dfl s =
+    p s (fun x _ -> donea x) (fun _ -> dfl)
+      (fun sa _ _ -> run_parse p donea dfl sa);;
+
+let rec make
+  program_content program_length =
+    Program_ext (program_content, program_length, ());;
+
+let rec int_to_bytes
+  n = (let na =
+         divide_int n
+           (Pos (Bit0 (Bit0 (Bit0 (Bit0 (Bit0 (Bit0 (Bit0 (Bit0 One)))))))))
+         in
+       let mo =
+         modulo_int n
+           (Pos (Bit0 (Bit0 (Bit0 (Bit0 (Bit0 (Bit0 (Bit0 (Bit0 One)))))))))
+         in
+        (if equal_inta na Zero_int then [byteFromNat (nat mo)]
+          else byteFromNat (nat mo) :: int_to_bytes na));;
+
+let rec intToBytes i = rev (int_to_bytes i);;
+
+let rec word160FromNatural
+  i = word_of_int
+        (len0_bit0
+          (len0_bit0
+            (len0_bit0
+              (len0_bit0 (len0_bit0 (len0_bit1 (len0_bit0 len0_num1)))))))
+        (of_nat semiring_1_int i);;
+
+let w160_0 : num1 bit0 bit1 bit0 bit0 bit0 bit0 bit0 word
+  = word160FromNatural Zero_nat;;
+
+let rec stree_append x0 uu = match x0, uu with STStr x, uu -> STStr x
+                       | STStrs xs, s -> STStrs (xs @ [s]);;
+
+let rec llll_parse
+  x0 uu uv uw ux = match x0, uu, uv, uw, ux with [], uu, uv, uw, ux -> None
+    | h :: t, token, parsed, isComment, isQuote ->
+        (if isComment
+          then (if equal_chara h newline
+                 then (if not (null token)
+                        then (match parsed with [] -> None
+                               | ph :: pt ->
+                                 llll_parse t []
+                                   (stree_append ph (STStr token) :: pt) false
+                                   false)
+                        else llll_parse t [] parsed false false)
+                 else llll_parse t token parsed true false)
+          else (if isQuote
+                 then (if equal_chara h quote
+                        then (if null token then None
+                               else (match parsed with [] -> None
+                                      | ph :: pt ->
+llll_parse t [] (stree_append ph (STStr (token @ [h])) :: pt) false false))
+                        else llll_parse t (token @ [h]) parsed false true)
+                 else (if equal_chara h
+                            (Chara
+                              (true, true, false, true, true, true, false,
+                                false))
+                        then llll_parse t token parsed true false
+                        else (if equal_chara h quote
+                               then llll_parse t (token @ [h]) parsed false true
+                               else (if equal_chara h
+  (Chara (false, false, false, true, false, true, false, false))
+                                      then llll_parse t token
+     (STStrs [] :: parsed) false false
+                                      else (if equal_chara h
+         (Chara (true, false, false, true, false, true, false, false))
+     then (match parsed with [] -> None
+            | [ph] ->
+              (if not (null token) then Some (stree_append ph (STStr token))
+                else Some ph)
+            | ph :: ph2 :: pt ->
+              (if not (null token)
+                then llll_parse t []
+                       (stree_append ph2 (stree_append ph (STStr token)) :: pt)
+                       false false
+                else llll_parse t [] (stree_append ph2 ph :: pt) false false))
+     else (if isWs h
+            then (if not (null token)
+                   then (match parsed with [] -> None
+                          | ph :: pt ->
+                            llll_parse t []
+                              (stree_append ph (STStr token) :: pt) false false)
+                   else llll_parse t [] parsed false false)
+            else llll_parse t (token @ [h]) parsed false false)))))));;
+
+let rec llll_parse0 s = llll_parse s [] [] false false;;
+
+let rec run_parse_opt p f s = run_parse p f None s;;
+
+let rec run_parse_opta p s = run_parse_opt p (fun a -> Some a) s;;
+
+let rec parseStringChar
+  x0 s f r = match x0, s, f, r with [], s, f, r -> f []
+    | h :: t, s, f, r -> (if equal_chara h quote then f (h :: t) else s [h] t);;
+
+let rec parseStringSub
+  s x1 su fa r = match s, x1, su, fa, r with s, [], su, fa, r -> fa []
+    | s, h :: t, su, fa, r ->
+        (if equal_chara h quote then (if null s then fa (h :: t) else su s t)
+          else parseStringChar (h :: t)
+                 (fun nextc l -> parseStringSub (s @ nextc) l su fa r) fa r);;
+
+let rec parseString
+  x0 su fa r = match x0, su, fa, r with [], su, fa, r -> fa []
+    | h :: t, su, fa, r ->
+        (if equal_chara h quote
+          then parseStringChar t (fun s l -> parseStringSub s l su fa r) fa r
+          else fa (h :: t));;
+
+let rec llll_parse1
+  ft x1 = match ft, x1 with
+    ft, STStr s ->
+      (match run_parse_opta parseHex s
+        with None ->
+          (match run_parse_opta parseInt s
+            with None ->
+              (match run_parse_opta parseString s
+                with None ->
+                  (match lookupS ft s with None -> None
+                    | Some f ->
+                      (match f [] with None -> None
+                        | Some l -> Some (l, (None, ft))))
+                | Some sa -> Some (L4L_Str sa, (None, ft)))
+            | Some n -> Some (L4L_Int n, (None, ft)))
+        | Some n -> Some (L4L_Int n, (None, ft)))
+    | ft, STStrs (h :: t) ->
+        (match h
+          with STStr hs ->
+            (if equal_lista equal_char hs
+                  [Chara (false, false, true, false, false, true, true, false);
+                    Chara (true, false, true, false, false, true, true, false);
+                    Chara (false, true, true, false, false, true, true, false)]
+              then (match t with [] -> None | [STStr _] -> None
+                     | [STStr h2; STStr listaa] ->
+                       (match llll_parse1_def h2 ft [] [STStr listaa]
+                         with None -> None | Some a -> Some a)
+                     | STStr _ :: STStr _ :: _ :: _ -> None
+                     | [STStr h2; STStrs l] ->
+                       (match llll_parse1_def h2 ft [] [STStrs l]
+                         with None -> None | Some a -> Some a)
+                     | [STStr h2; STStrs l; d] ->
+                       (match llll_parse1_def h2 ft [] (l @ [d])
+                         with None -> None | Some a -> Some a)
+                     | STStr _ :: STStrs _ :: _ :: _ :: _ -> None
+                     | STStrs _ :: _ -> None)
+              else (if equal_lista equal_char hs
+                         [Chara (false, true, false, false, true, true, true,
+                                  false);
+                           Chara (true, false, true, false, false, true, true,
+                                   false);
+                           Chara (false, false, true, false, true, true, true,
+                                   false);
+                           Chara (true, false, true, false, true, true, true,
+                                   false);
+                           Chara (false, true, false, false, true, true, true,
+                                   false);
+                           Chara (false, true, true, true, false, true, true,
+                                   false);
+                           Chara (false, false, true, true, false, true, true,
+                                   false);
+                           Chara (false, false, true, true, false, true, true,
+                                   false);
+                           Chara (false, false, true, true, false, true, true,
+                                   false)]
+                     then (match t with [] -> None
+                            | [paysrc] ->
+                              (match llll_parse1 ft paysrc with None -> None
+                                | Some (ls, (None, fta)) ->
+                                  Some (L4Seq [], (Some ls, fta))
+                                | Some (_, (Some _, _)) -> None)
+                            | _ :: _ :: _ -> None)
+                     else (match lookupS ft hs with None -> None
+                            | Some f ->
+                              (match llll_parse1_args ft t with None -> None
+                                | Some (ls, (x, fta)) ->
+                                  (match f ls with None -> None
+                                    | Some l -> Some (l, (x, fta)))))))
+          | STStrs _ -> None)
+    | ft, STStrs [] -> None
+and llll_parse1_def
+  s ft vt x3 = match s, ft, vt, x3 with s, ft, vt, [] -> None
+    | name, ft, vt, [h] ->
+        (match name with [] -> None | [_] -> None
+          | hdchr :: aa :: lista ->
+            (if not (equal_chara hdchr apos) then None
+              else Some (L4Seq [],
+                          (None,
+                            (aa :: lista,
+                              (fun l ->
+                                (match mkConsts vt (rev l) with None -> None
+                                  | Some fta ->
+                                    (match llll_parse1 (fta @ ft) h
+                                      with None -> None
+                                      | Some (la, (_, _)) -> Some la)))) ::
+                              ft))))
+    | name, ft, vt, h :: v :: va ->
+        (match h with STStr vb -> llll_parse1_def name ft (vb :: vt) (v :: va)
+          | STStrs _ -> None)
+and llll_parse1_args
+  ft x1 = match ft, x1 with ft, [] -> Some ([], (None, ft))
+    | ft, [h] ->
+        (match llll_parse1 ft h with None -> None
+          | Some (l, (x, fta)) -> Some ([l], (x, fta)))
+    | ft, h :: v :: va ->
+        (match llll_parse1 ft h with None -> None
+          | Some (ha, (None, fta)) ->
+            (match llll_parse1_args fta (v :: va) with None -> None
+              | Some (t, (x, ftb)) -> Some (ha :: t, (x, ftb)))
+          | Some (ha, (Some pay, fta)) -> Some ([ha], (Some pay, fta)));;
+
+let rec makeLogical i = [i; L (Arith ISZERO); L (Arith ISZERO)];;
+
+let rec minus_nat m n = match m, n with Suc m, Suc n -> minus_nat m n
+                    | Zero_nat, n -> Zero_nat
+                    | m, Zero_nat -> m;;
+
+let rec divmod_nat
+  m n = (if equal_nata n Zero_nat || less_nat m n then (Zero_nat, m)
+          else (let a = divmod_nat (minus_nat m n) n in
+                let (q, aa) = a in
+                 (Suc q, aa)));;
+
+let rec mynth x0 uu = match x0, uu with [], uu -> None
+                | h :: t, Zero_nat -> h
+                | h :: t, Suc v -> mynth t (minus_nat (Suc v) one_nat);;
+
+let rec hexwrite1
+  c = (if equal_nata c Zero_nat
+        then Chara (false, false, false, false, true, true, false, false)
+        else (if equal_nata c one_nat
+               then Chara (true, false, false, false, true, true, false, false)
+               else (if equal_nata c (nat_of_num (Bit0 One))
+                      then Chara (false, true, false, false, true, true, false,
+                                   false)
+                      else (if equal_nata c (nat_of_num (Bit1 One))
+                             then Chara (true, true, false, false, true, true,
+  false, false)
+                             else (if equal_nata c
+(nat_of_num (Bit0 (Bit0 One)))
+                                    then Chara
+   (false, false, true, false, true, true, false, false)
+                                    else (if equal_nata c
+       (nat_of_num (Bit1 (Bit0 One)))
+   then Chara (true, false, true, false, true, true, false, false)
+   else (if equal_nata c (nat_of_num (Bit0 (Bit1 One)))
+          then Chara (false, true, true, false, true, true, false, false)
+          else (if equal_nata c (nat_of_num (Bit1 (Bit1 One)))
+                 then Chara (true, true, true, false, true, true, false, false)
+                 else (if equal_nata c (nat_of_num (Bit0 (Bit0 (Bit0 One))))
+                        then Chara (false, false, false, true, true, true,
+                                     false, false)
+                        else (if equal_nata c
+                                   (nat_of_num (Bit1 (Bit0 (Bit0 One))))
+                               then Chara (true, false, false, true, true, true,
+    false, false)
+                               else (if equal_nata c
+  (nat_of_num (Bit0 (Bit1 (Bit0 One))))
+                                      then Chara
+     (true, false, false, false, false, true, true, false)
+                                      else (if equal_nata c
+         (nat_of_num (Bit1 (Bit1 (Bit0 One))))
+     then Chara (false, true, false, false, false, true, true, false)
+     else (if equal_nata c (nat_of_num (Bit0 (Bit0 (Bit1 One))))
+            then Chara (true, true, false, false, false, true, true, false)
+            else (if equal_nata c (nat_of_num (Bit1 (Bit0 (Bit1 One))))
+                   then Chara (false, false, true, false, false, true, true,
+                                false)
+                   else (if equal_nata c (nat_of_num (Bit0 (Bit1 (Bit1 One))))
+                          then Chara (true, false, true, false, false, true,
+                                       true, false)
+                          else (if equal_nata c
+                                     (nat_of_num (Bit1 (Bit1 (Bit1 One))))
+                                 then Chara
+(false, true, true, false, false, true, true, false)
+                                 else failwith "undefined"))))))))))))))));;
+
+let rec hexwrite2
+  w = (let (d, m) =
+         divmod_nat (unat (len0_bit0 (len0_bit0 (len0_bit0 len0_num1))) w)
+           (nat_of_num (Bit0 (Bit0 (Bit0 (Bit0 One)))))
+         in
+        (hexwrite1 d, hexwrite1 m));;
+
+let rec hexwrite
+  = function [] -> []
+    | h :: t -> (let (c1, c2) = hexwrite2 h in c1 :: c2 :: hexwrite t);;
+
+let rec program_of_lst
+  lst program_content_formatter =
+    Program_ext
+      (program_content_formatter lst, of_nat semiring_1_int (size_list lst),
+        ());;
 
 let rec sgn_integer
   k = (if Big_int.eq_big_int k Big_int.zero_big_int then Big_int.zero_big_int
@@ -199,722 +1489,99 @@ let rec divmod_integer
    (Big_int.minus_big_int r) (Big_int.big_int_of_int 1),
   Big_int.sub_big_int (Big_int.abs_big_int l) s))))));;
 
-let rec snd (x1, x2) = x2;;
-
-let rec modulo_integer k l = snd (divmod_integer k l);;
-
-let rec modulo_int
-  k l = Int_of_integer (modulo_integer (integer_of_int k) (integer_of_int l));;
-
-let rec minus_nat
-  m n = Nat (max ord_integer Big_int.zero_big_int
-              (Big_int.sub_big_int (integer_of_nat m) (integer_of_nat n)));;
-
-let rec equal_nat
-  m n = Big_int.eq_big_int (integer_of_nat m) (integer_of_nat n);;
-
-let rec power _A
-  a n = (if equal_nat n zero_nat then one _A.one_power
-          else times _A.times_power a (power _A a (minus_nat n one_nat)));;
-
-let rec word_of_int _A
-  k = Word (modulo_int k
-             (power power_int (Int_of_integer (Big_int.big_int_of_int 2))
-               (len_of _A Type)));;
-
-let rec storage_inst_code
-  = function
-    SLOAD ->
-      word_of_int (len0_bit0 (len0_bit0 (len0_bit0 len0_num1)))
-        (Int_of_integer (Big_int.big_int_of_int 84))
-    | SSTORE ->
-        word_of_int (len0_bit0 (len0_bit0 (len0_bit0 len0_num1)))
-          (Int_of_integer (Big_int.big_int_of_int 85));;
-
-let rec sarith_inst_code
-  = function
-    SDIV ->
-      word_of_int (len0_bit0 (len0_bit0 (len0_bit0 len0_num1)))
-        (Int_of_integer (Big_int.big_int_of_int 5))
-    | SMOD ->
-        word_of_int (len0_bit0 (len0_bit0 (len0_bit0 len0_num1)))
-          (Int_of_integer (Big_int.big_int_of_int 7))
-    | SGT ->
-        word_of_int (len0_bit0 (len0_bit0 (len0_bit0 len0_num1)))
-          (Int_of_integer (Big_int.big_int_of_int 19))
-    | SLT ->
-        word_of_int (len0_bit0 (len0_bit0 (len0_bit0 len0_num1)))
-          (Int_of_integer (Big_int.big_int_of_int 18))
-    | SIGNEXTEND ->
-        word_of_int (len0_bit0 (len0_bit0 (len0_bit0 len0_num1)))
-          (Int_of_integer (Big_int.big_int_of_int 11));;
-
-let rec memory_inst_code
-  = function
-    MLOAD ->
-      word_of_int (len0_bit0 (len0_bit0 (len0_bit0 len0_num1)))
-        (Int_of_integer (Big_int.big_int_of_int 81))
-    | MSTORE ->
-        word_of_int (len0_bit0 (len0_bit0 (len0_bit0 len0_num1)))
-          (Int_of_integer (Big_int.big_int_of_int 82))
-    | MSTORE8 ->
-        word_of_int (len0_bit0 (len0_bit0 (len0_bit0 len0_num1)))
-          (Int_of_integer (Big_int.big_int_of_int 83))
-    | CALLDATACOPY ->
-        word_of_int (len0_bit0 (len0_bit0 (len0_bit0 len0_num1)))
-          (Int_of_integer (Big_int.big_int_of_int 55))
-    | CODECOPY ->
-        word_of_int (len0_bit0 (len0_bit0 (len0_bit0 len0_num1)))
-          (Int_of_integer (Big_int.big_int_of_int 57))
-    | EXTCODECOPY ->
-        word_of_int (len0_bit0 (len0_bit0 (len0_bit0 len0_num1)))
-          (Int_of_integer (Big_int.big_int_of_int 60))
-    | MSIZE ->
-        word_of_int (len0_bit0 (len0_bit0 (len0_bit0 len0_num1)))
-          (Int_of_integer (Big_int.big_int_of_int 89));;
-
-let rec plus_int
-  k l = Int_of_integer
-          (Big_int.add_big_int (integer_of_int k) (integer_of_int l));;
-
-let rec plus_word _A a b = word_of_int _A (plus_int (uint _A a) (uint _A b));;
-
-let zero_int : int = Int_of_integer Big_int.zero_big_int;;
-
-let rec less_nat
-  m n = Big_int.lt_big_int (integer_of_nat m) (integer_of_nat n);;
-
-let rec word8FromNat
-  i = word_of_int (len0_bit0 (len0_bit0 (len0_bit0 len0_num1))) (int_of_nat i);;
-
-let rec byteFromNat x = word8FromNat x;;
-
-let rec stack_inst_code
-  = function
-    POP ->
-      [word_of_int (len0_bit0 (len0_bit0 (len0_bit0 len0_num1)))
-         (Int_of_integer (Big_int.big_int_of_int 80))]
-    | PUSH_N lst ->
-        (if less_nat (size_list lst) one_nat
-          then [word_of_int (len0_bit0 (len0_bit0 (len0_bit0 len0_num1)))
-                  (Int_of_integer (Big_int.big_int_of_int 96));
-                 word_of_int (len0_bit0 (len0_bit0 (len0_bit0 len0_num1)))
-                   zero_int]
-          else (if less_nat (nat_of_integer (Big_int.big_int_of_int 32))
-                     (size_list lst)
-                 then [word_of_int (len0_bit0 (len0_bit0 (len0_bit0 len0_num1)))
-                         (Int_of_integer (Big_int.big_int_of_int 96));
-                        word_of_int
-                          (len0_bit0 (len0_bit0 (len0_bit0 len0_num1)))
-                          zero_int]
-                 else [plus_word (len0_bit0 (len0_bit0 (len0_bit0 len0_num1)))
-                         (byteFromNat (size_list lst))
-                         (word_of_int
-                           (len0_bit0 (len0_bit0 (len0_bit0 len0_num1)))
-                           (Int_of_integer (Big_int.big_int_of_int 95)))] @
-                        lst))
-    | CALLDATALOAD ->
-        [word_of_int (len0_bit0 (len0_bit0 (len0_bit0 len0_num1)))
-           (Int_of_integer (Big_int.big_int_of_int 53))];;
-
-let rec arith_inst_code
-  = function
-    ADD -> word_of_int (len0_bit0 (len0_bit0 (len0_bit0 len0_num1))) one_inta
-    | MUL ->
-        word_of_int (len0_bit0 (len0_bit0 (len0_bit0 len0_num1)))
-          (Int_of_integer (Big_int.big_int_of_int 2))
-    | SUB ->
-        word_of_int (len0_bit0 (len0_bit0 (len0_bit0 len0_num1)))
-          (Int_of_integer (Big_int.big_int_of_int 3))
-    | DIV ->
-        word_of_int (len0_bit0 (len0_bit0 (len0_bit0 len0_num1)))
-          (Int_of_integer (Big_int.big_int_of_int 4))
-    | MOD ->
-        word_of_int (len0_bit0 (len0_bit0 (len0_bit0 len0_num1)))
-          (Int_of_integer (Big_int.big_int_of_int 6))
-    | ADDMOD ->
-        word_of_int (len0_bit0 (len0_bit0 (len0_bit0 len0_num1)))
-          (Int_of_integer (Big_int.big_int_of_int 8))
-    | MULMOD ->
-        word_of_int (len0_bit0 (len0_bit0 (len0_bit0 len0_num1)))
-          (Int_of_integer (Big_int.big_int_of_int 9))
-    | EXP ->
-        word_of_int (len0_bit0 (len0_bit0 (len0_bit0 len0_num1)))
-          (Int_of_integer (Big_int.big_int_of_int 10))
-    | Inst_GT ->
-        word_of_int (len0_bit0 (len0_bit0 (len0_bit0 len0_num1)))
-          (Int_of_integer (Big_int.big_int_of_int 17))
-    | Inst_LT ->
-        word_of_int (len0_bit0 (len0_bit0 (len0_bit0 len0_num1)))
-          (Int_of_integer (Big_int.big_int_of_int 16))
-    | Inst_EQ ->
-        word_of_int (len0_bit0 (len0_bit0 (len0_bit0 len0_num1)))
-          (Int_of_integer (Big_int.big_int_of_int 20))
-    | ISZERO ->
-        word_of_int (len0_bit0 (len0_bit0 (len0_bit0 len0_num1)))
-          (Int_of_integer (Big_int.big_int_of_int 21))
-    | SHA3 ->
-        word_of_int (len0_bit0 (len0_bit0 (len0_bit0 len0_num1)))
-          (Int_of_integer (Big_int.big_int_of_int 32));;
-
-let rec swap_inst_code
-  m = plus_word (len0_bit0 (len0_bit0 (len0_bit0 len0_num1)))
-        (word_of_int (len0_bit0 (len0_bit0 (len0_bit0 len0_num1)))
-          (uint (len0_bit0 (len0_bit0 len0_num1)) m))
-        (word_of_int (len0_bit0 (len0_bit0 (len0_bit0 len0_num1)))
-          (Int_of_integer (Big_int.big_int_of_int 144)));;
-
-let rec misc_inst_code
-  = function
-    STOP -> word_of_int (len0_bit0 (len0_bit0 (len0_bit0 len0_num1))) zero_int
-    | CREATE ->
-        word_of_int (len0_bit0 (len0_bit0 (len0_bit0 len0_num1)))
-          (Int_of_integer (Big_int.big_int_of_int 240))
-    | CALL ->
-        word_of_int (len0_bit0 (len0_bit0 (len0_bit0 len0_num1)))
-          (Int_of_integer (Big_int.big_int_of_int 241))
-    | CALLCODE ->
-        word_of_int (len0_bit0 (len0_bit0 (len0_bit0 len0_num1)))
-          (Int_of_integer (Big_int.big_int_of_int 242))
-    | RETURN ->
-        word_of_int (len0_bit0 (len0_bit0 (len0_bit0 len0_num1)))
-          (Int_of_integer (Big_int.big_int_of_int 243))
-    | DELEGATECALL ->
-        word_of_int (len0_bit0 (len0_bit0 (len0_bit0 len0_num1)))
-          (Int_of_integer (Big_int.big_int_of_int 244))
-    | SUICIDE ->
-        word_of_int (len0_bit0 (len0_bit0 (len0_bit0 len0_num1)))
-          (Int_of_integer (Big_int.big_int_of_int 255));;
-
-let rec info_inst_code
-  = function
-    ADDRESS ->
-      word_of_int (len0_bit0 (len0_bit0 (len0_bit0 len0_num1)))
-        (Int_of_integer (Big_int.big_int_of_int 48))
-    | BALANCE ->
-        word_of_int (len0_bit0 (len0_bit0 (len0_bit0 len0_num1)))
-          (Int_of_integer (Big_int.big_int_of_int 49))
-    | ORIGIN ->
-        word_of_int (len0_bit0 (len0_bit0 (len0_bit0 len0_num1)))
-          (Int_of_integer (Big_int.big_int_of_int 50))
-    | CALLVALUE ->
-        word_of_int (len0_bit0 (len0_bit0 (len0_bit0 len0_num1)))
-          (Int_of_integer (Big_int.big_int_of_int 52))
-    | CALLDATASIZE ->
-        word_of_int (len0_bit0 (len0_bit0 (len0_bit0 len0_num1)))
-          (Int_of_integer (Big_int.big_int_of_int 54))
-    | CALLER ->
-        word_of_int (len0_bit0 (len0_bit0 (len0_bit0 len0_num1)))
-          (Int_of_integer (Big_int.big_int_of_int 51))
-    | CODESIZE ->
-        word_of_int (len0_bit0 (len0_bit0 (len0_bit0 len0_num1)))
-          (Int_of_integer (Big_int.big_int_of_int 56))
-    | GASPRICE ->
-        word_of_int (len0_bit0 (len0_bit0 (len0_bit0 len0_num1)))
-          (Int_of_integer (Big_int.big_int_of_int 58))
-    | EXTCODESIZE ->
-        word_of_int (len0_bit0 (len0_bit0 (len0_bit0 len0_num1)))
-          (Int_of_integer (Big_int.big_int_of_int 59))
-    | BLOCKHASH ->
-        word_of_int (len0_bit0 (len0_bit0 (len0_bit0 len0_num1)))
-          (Int_of_integer (Big_int.big_int_of_int 64))
-    | COINBASE ->
-        word_of_int (len0_bit0 (len0_bit0 (len0_bit0 len0_num1)))
-          (Int_of_integer (Big_int.big_int_of_int 65))
-    | TIMESTAMP ->
-        word_of_int (len0_bit0 (len0_bit0 (len0_bit0 len0_num1)))
-          (Int_of_integer (Big_int.big_int_of_int 66))
-    | NUMBER ->
-        word_of_int (len0_bit0 (len0_bit0 (len0_bit0 len0_num1)))
-          (Int_of_integer (Big_int.big_int_of_int 67))
-    | DIFFICULTY ->
-        word_of_int (len0_bit0 (len0_bit0 (len0_bit0 len0_num1)))
-          (Int_of_integer (Big_int.big_int_of_int 68))
-    | GASLIMIT ->
-        word_of_int (len0_bit0 (len0_bit0 (len0_bit0 len0_num1)))
-          (Int_of_integer (Big_int.big_int_of_int 69))
-    | GAS ->
-        word_of_int (len0_bit0 (len0_bit0 (len0_bit0 len0_num1)))
-          (Int_of_integer (Big_int.big_int_of_int 90));;
-
-let rec bits_inst_code
-  = function
-    Inst_AND ->
-      word_of_int (len0_bit0 (len0_bit0 (len0_bit0 len0_num1)))
-        (Int_of_integer (Big_int.big_int_of_int 22))
-    | Inst_OR ->
-        word_of_int (len0_bit0 (len0_bit0 (len0_bit0 len0_num1)))
-          (Int_of_integer (Big_int.big_int_of_int 23))
-    | Inst_XOR ->
-        word_of_int (len0_bit0 (len0_bit0 (len0_bit0 len0_num1)))
-          (Int_of_integer (Big_int.big_int_of_int 24))
-    | Inst_NOT ->
-        word_of_int (len0_bit0 (len0_bit0 (len0_bit0 len0_num1)))
-          (Int_of_integer (Big_int.big_int_of_int 25))
-    | BYTE ->
-        word_of_int (len0_bit0 (len0_bit0 (len0_bit0 len0_num1)))
-          (Int_of_integer (Big_int.big_int_of_int 26));;
-
-let rec log_inst_code
-  = function
-    LOG0 ->
-      word_of_int (len0_bit0 (len0_bit0 (len0_bit0 len0_num1)))
-        (Int_of_integer (Big_int.big_int_of_int 160))
-    | LOG1 ->
-        word_of_int (len0_bit0 (len0_bit0 (len0_bit0 len0_num1)))
-          (Int_of_integer (Big_int.big_int_of_int 161))
-    | LOG2 ->
-        word_of_int (len0_bit0 (len0_bit0 (len0_bit0 len0_num1)))
-          (Int_of_integer (Big_int.big_int_of_int 162))
-    | LOG3 ->
-        word_of_int (len0_bit0 (len0_bit0 (len0_bit0 len0_num1)))
-          (Int_of_integer (Big_int.big_int_of_int 163))
-    | LOG4 ->
-        word_of_int (len0_bit0 (len0_bit0 (len0_bit0 len0_num1)))
-          (Int_of_integer (Big_int.big_int_of_int 164));;
-
-let rec dup_inst_code
-  m = plus_word (len0_bit0 (len0_bit0 (len0_bit0 len0_num1)))
-        (word_of_int (len0_bit0 (len0_bit0 (len0_bit0 len0_num1)))
-          (uint (len0_bit0 (len0_bit0 len0_num1)) m))
-        (word_of_int (len0_bit0 (len0_bit0 (len0_bit0 len0_num1)))
-          (Int_of_integer (Big_int.big_int_of_int 128)));;
-
-let rec pc_inst_code
-  = function
-    JUMP ->
-      word_of_int (len0_bit0 (len0_bit0 (len0_bit0 len0_num1)))
-        (Int_of_integer (Big_int.big_int_of_int 86))
-    | JUMPI ->
-        word_of_int (len0_bit0 (len0_bit0 (len0_bit0 len0_num1)))
-          (Int_of_integer (Big_int.big_int_of_int 87))
-    | PC -> word_of_int (len0_bit0 (len0_bit0 (len0_bit0 len0_num1)))
-              (Int_of_integer (Big_int.big_int_of_int 88))
-    | JUMPDEST ->
-        word_of_int (len0_bit0 (len0_bit0 (len0_bit0 len0_num1)))
-          (Int_of_integer (Big_int.big_int_of_int 91));;
-
-let rec inst_code = function Unknown byte -> [byte]
-                    | Bits b -> [bits_inst_code b]
-                    | Sarith s -> [sarith_inst_code s]
-                    | Arith a -> [arith_inst_code a]
-                    | Info i -> [info_inst_code i]
-                    | Dup d -> [dup_inst_code d]
-                    | Memory m -> [memory_inst_code m]
-                    | Storage s -> [storage_inst_code s]
-                    | Pc p -> [pc_inst_code p]
-                    | Stack s -> stack_inst_code s
-                    | Swap s -> [swap_inst_code s]
-                    | Log l -> [log_inst_code l]
-                    | Misc m -> [misc_inst_code m];;
-
-let rec inst_size i = int_of_nat (size_list (inst_code i));;
-
-let rec ilsz = function [] -> zero_nat
-               | h :: t -> plus_nat (nat (inst_size h)) (ilsz t);;
-
-let rec map f x1 = match f, x1 with f, [] -> []
-              | f, x21 :: x22 -> f x21 :: map f x22;;
-
-let rec member _A x0 y = match x0, y with [], y -> false
-                    | x :: xs, y -> eq _A x y || member _A xs y;;
-
-let rec isWs
-  x = member equal_char
-        (map char_of_nat
-          [nat_of_integer (Big_int.big_int_of_int 9);
-            nat_of_integer (Big_int.big_int_of_int 10);
-            nat_of_integer (Big_int.big_int_of_int 11);
-            nat_of_integer (Big_int.big_int_of_int 12);
-            nat_of_integer (Big_int.big_int_of_int 13);
-            nat_of_integer (Big_int.big_int_of_int 32)])
-        x;;
-
-let rec foldl f a x2 = match f, a, x2 with f, a, [] -> a
-                | f, a, x :: xs -> foldl f (f a x) xs;;
-
-let rec map_of _A
-  x0 k = match x0, k with
-    (l, v) :: ps, k -> (if eq _A l k then Some v else map_of _A ps k)
-    | [], k -> None;;
-
-let rec il2wl il = maps inst_code il;;
-
-let rec equal_list _A
-  x0 x1 = match x0, x1 with [], x21 :: x22 -> false
-    | x21 :: x22, [] -> false
-    | x21 :: x22, y21 :: y22 -> eq _A x21 y21 && equal_list _A x22 y22
-    | [], [] -> true;;
-
-let rec lookupS
-  x0 uu = match x0, uu with [], uu -> None
-    | (ah, bh) :: t, a ->
-        (if equal_list equal_char a ah then Some bh else lookupS t a);;
-
-let rec mkConsts
-  x0 x1 = match x0, x1 with [], [] -> Some []
-    | sh :: st, lh :: lt ->
-        (match mkConsts st lt with None -> None
-          | Some ft -> Some ((sh, (fun _ -> Some lh)) :: ft))
-    | v :: va, [] -> None
-    | [], v :: va -> None;;
-
-let hex_parse_table : (char * nat) list
-  = [('0', zero_nat); ('1', one_nat);
-      ('2', nat_of_integer (Big_int.big_int_of_int 2));
-      ('3', nat_of_integer (Big_int.big_int_of_int 3));
-      ('4', nat_of_integer (Big_int.big_int_of_int 4));
-      ('5', nat_of_integer (Big_int.big_int_of_int 5));
-      ('6', nat_of_integer (Big_int.big_int_of_int 6));
-      ('7', nat_of_integer (Big_int.big_int_of_int 7));
-      ('8', nat_of_integer (Big_int.big_int_of_int 8));
-      ('9', nat_of_integer (Big_int.big_int_of_int 9));
-      ('A', nat_of_integer (Big_int.big_int_of_int 10));
-      ('a', nat_of_integer (Big_int.big_int_of_int 10));
-      ('B', nat_of_integer (Big_int.big_int_of_int 11));
-      ('b', nat_of_integer (Big_int.big_int_of_int 11));
-      ('C', nat_of_integer (Big_int.big_int_of_int 12));
-      ('c', nat_of_integer (Big_int.big_int_of_int 12));
-      ('D', nat_of_integer (Big_int.big_int_of_int 13));
-      ('d', nat_of_integer (Big_int.big_int_of_int 13));
-      ('E', nat_of_integer (Big_int.big_int_of_int 14));
-      ('e', nat_of_integer (Big_int.big_int_of_int 14));
-      ('F', nat_of_integer (Big_int.big_int_of_int 15));
-      ('f', nat_of_integer (Big_int.big_int_of_int 15))];;
-
-let rec parseHexNumeral
-  x0 s f r = match x0, s, f, r with [], s, f, r -> f []
-    | h :: t, s, f, r ->
-        (match map_of equal_char hex_parse_table h with None -> f (h :: t)
-          | Some n -> s n t);;
-
-let rec parseHexSub
-  i x1 su fa r = match i, x1, su, fa, r with i, [], su, fa, r -> su i []
-    | i, h :: t, su, fa, r ->
-        parseHexNumeral (h :: t)
-          (fun n l ->
-            parseHexSub
-              (plus_nat
-                (times_nat (nat_of_integer (Big_int.big_int_of_int 16)) i) n)
-              l su fa r)
-          (su i) r;;
-
-let rec parseHex
-  x0 su fa r = match x0, su, fa, r with
-    h0 :: hx :: h :: t, su, fa, r ->
-      (if ((h0 : char) = '0') && ((hx : char) = 'x')
-        then parseHexNumeral (h :: t) (fun n l -> parseHexSub n l su fa r) fa r
-        else fa (h0 :: hx :: h :: t))
-    | [], su, fa, r -> fa []
-    | [v], su, fa, r -> fa [v]
-    | [v; vb], su, fa, r -> fa [v; vb];;
-
-let rec is_digit_char
-  c = ((c : char) = '0') ||
-        (((c : char) = '5') ||
-          (((c : char) = '1') ||
-            (((c : char) = '6') ||
-              (((c : char) = '2') ||
-                (((c : char) = '7') ||
-                  (((c : char) = '3') ||
-                    (((c : char) = '8') ||
-                      (((c : char) = '4') || ((c : char) = '9')))))))));;
-
-let rec char_to_digit
-  c = (if ((c : char) = '0') then zero_nat
-        else (if ((c : char) = '1') then one_nat
-               else (if ((c : char) = '2')
-                      then nat_of_integer (Big_int.big_int_of_int 2)
-                      else (if ((c : char) = '3')
-                             then nat_of_integer (Big_int.big_int_of_int 3)
-                             else (if ((c : char) = '4')
-                                    then nat_of_integer
-   (Big_int.big_int_of_int 4)
-                                    else (if ((c : char) = '5')
-   then nat_of_integer (Big_int.big_int_of_int 5)
-   else (if ((c : char) = '6') then nat_of_integer (Big_int.big_int_of_int 6)
-          else (if ((c : char) = '7')
-                 then nat_of_integer (Big_int.big_int_of_int 7)
-                 else (if ((c : char) = '8')
-                        then nat_of_integer (Big_int.big_int_of_int 8)
-                        else (if ((c : char) = '9')
-                               then nat_of_integer (Big_int.big_int_of_int 9)
-                               else nat_of_integer
-                                      (Big_int.big_int_of_int 10)))))))))));;
-
-let rec parseNumeral
-  x0 s f r = match x0, s, f, r with [], s, f, r -> f []
-    | h :: t, s, f, r ->
-        (if is_digit_char h then s (char_to_digit h) t else f (h :: t));;
-
-let rec parseNatSub
-  i x1 su fa r = match i, x1, su, fa, r with i, [], su, fa, r -> su i []
-    | i, h :: t, su, fa, r ->
-        parseNumeral (h :: t)
-          (fun n l ->
-            parseNatSub
-              (plus_nat
-                (times_nat (nat_of_integer (Big_int.big_int_of_int 10)) i) n)
-              l su fa r)
-          (su i) r;;
-
-let rec parseNat
-  x0 su fa r = match x0, su, fa, r with [], su, fa, r -> fa []
-    | h :: t, su, fa, r ->
-        parseNumeral (h :: t) (fun n l -> parseNatSub n l su fa r) fa r;;
-
-let rec fst (x1, x2) = x1;;
-
-let rec divide_integer k l = fst (divmod_integer k l);;
-
-let rec divide_int
-  k l = Int_of_integer (divide_integer (integer_of_int k) (integer_of_int l));;
-
-let rec less_eq_int
-  k l = Big_int.le_big_int (integer_of_int k) (integer_of_int l);;
-
-let rec log256floor
-  x = (if less_eq_int x (Int_of_integer (Big_int.big_int_of_int 255))
-        then zero_int
-        else plus_int one_inta
-               (log256floor
-                 (divide_int x
-                   (Int_of_integer (Big_int.big_int_of_int 256)))));;
-
-let rec run_parse
-  p donea dfl s =
-    p s (fun x _ -> donea x) (fun _ -> dfl)
-      (fun sa _ _ -> run_parse p donea dfl sa);;
-
-let rec modulo_nat
-  m n = Nat (modulo_integer (integer_of_nat m) (integer_of_nat n));;
-
-let rec divide_nat
-  m n = Nat (divide_integer (integer_of_nat m) (integer_of_nat n));;
-
-let rec divmod_nat m n = (divide_nat m n, modulo_nat m n);;
-
-let rec nat_to_bytes
-  n = (let (a, mo) = divmod_nat n (nat_of_integer (Big_int.big_int_of_int 256))
-         in
-        (if equal_nat a zero_nat then [byteFromNat mo]
-          else byteFromNat mo :: nat_to_bytes (suc (minus_nat a one_nat))));;
-
-let rec output_address n = rev (nat_to_bytes n);;
-
-let rec intToBytes i = output_address (nat i);;
-
-let rec stree_append x0 uu = match x0, uu with STStr x, uu -> STStr x
-                       | STStrs xs, s -> STStrs (xs @ [s]);;
-
-let rec llll_parse
-  x0 uu uv = match x0, uu, uv with [], uu, uv -> None
-    | h :: t, token, parsed ->
-        (if ((h : char) = '(') then llll_parse t token (STStrs [] :: parsed)
-          else (if ((h : char) = ')')
-                 then (match parsed with [] -> None
-                        | [ph] ->
-                          (if not (null token)
-                            then Some (stree_append ph (STStr token))
-                            else Some ph)
-                        | ph :: ph2 :: pt ->
-                          (if not (null token)
-                            then llll_parse t []
-                                   (stree_append ph2
-                                      (stree_append ph (STStr token)) ::
-                                     pt)
-                            else llll_parse t [] (stree_append ph2 ph :: pt)))
-                 else (if isWs h
-                        then (if not (null token)
-                               then (match parsed with [] -> None
-                                      | ph :: pt ->
-llll_parse t [] (stree_append ph (STStr token) :: pt))
-                               else llll_parse t [] parsed)
-                        else llll_parse t (token @ [h]) parsed)));;
-
-let rec llll_parse0 s = llll_parse s [] [];;
-
-let rec run_parse_opt p f s = run_parse p f None s;;
-
-let rec run_parse_opta p s = run_parse_opt p (fun a -> Some a) s;;
-
-let rec llll_parse1
-  ft x1 = match ft, x1 with
-    ft, STStr s ->
-      (match run_parse_opta parseHex s
-        with None ->
-          (match run_parse_opta parseNat s
-            with None ->
-              (match lookupS ft s with None -> None
-                | Some f ->
-                  (match f [] with None -> None
-                    | Some l -> Some (l, (None, ft))))
-            | Some n -> Some (L4L_Nat n, (None, ft)))
-        | Some n -> Some (L4L_Nat n, (None, ft)))
-    | ft, STStrs (h :: t) ->
-        (match h
-          with STStr hs ->
-            (if equal_list equal_char hs ['d'; 'e'; 'f']
-              then (match t with [] -> None | [STStr _] -> None
-                     | [STStr h2; STStr listaa] ->
-                       (match llll_parse1_def h2 ft [] [STStr listaa]
-                         with None -> None | Some a -> Some a)
-                     | STStr _ :: STStr _ :: _ :: _ -> None
-                     | [STStr h2; STStrs l] ->
-                       (match llll_parse1_def h2 ft [] [STStrs l]
-                         with None -> None | Some a -> Some a)
-                     | [STStr h2; STStrs l; d] ->
-                       (match llll_parse1_def h2 ft [] (l @ [d])
-                         with None -> None | Some a -> Some a)
-                     | STStr _ :: STStrs _ :: _ :: _ :: _ -> None
-                     | STStrs _ :: _ -> None)
-              else (if equal_list equal_char hs
-                         ['r'; 'e'; 't'; 'u'; 'r'; 'n'; 'l'; 'l'; 'l']
-                     then (match t with [] -> None
-                            | [paysrc] ->
-                              (match llll_parse1 ft paysrc with None -> None
-                                | Some (ls, (None, fta)) ->
-                                  Some (L4Seq [], (Some ls, fta))
-                                | Some (_, (Some _, _)) -> None)
-                            | _ :: _ :: _ -> None)
-                     else (match lookupS ft hs with None -> None
-                            | Some f ->
-                              (match llll_parse1_args ft t with None -> None
-                                | Some (ls, (x, fta)) ->
-                                  (match f ls with None -> None
-                                    | Some l -> Some (l, (x, fta)))))))
-          | STStrs _ -> None)
-    | ft, STStrs [] -> None
-and llll_parse1_def
-  s ft vt x3 = match s, ft, vt, x3 with s, ft, vt, [] -> None
-    | name, ft, vt, [h] ->
-        (match name with [] -> None | [_] -> None
-          | hdchr :: aa :: lista ->
-            (if not ((hdchr : char) = apos) then None
-              else Some (L4Seq [],
-                          (None,
-                            (aa :: lista,
-                              (fun l ->
-                                (match mkConsts vt (rev l) with None -> None
-                                  | Some fta ->
-                                    (match llll_parse1 (fta @ ft) h
-                                      with None -> None
-                                      | Some (la, (_, _)) -> Some la)))) ::
-                              ft))))
-    | name, ft, vt, h :: v :: va ->
-        (match h with STStr vb -> llll_parse1_def name ft (vb :: vt) (v :: va)
-          | STStrs _ -> None)
-and llll_parse1_args
-  ft x1 = match ft, x1 with ft, [] -> None
-    | ft, [h] ->
-        (match llll_parse1 ft h with None -> None
-          | Some (l, (x, fta)) -> Some ([l], (x, fta)))
-    | ft, h :: v :: va ->
-        (match llll_parse1 ft h with None -> None
-          | Some (ha, (None, fta)) ->
-            (match llll_parse1_args fta (v :: va) with None -> None
-              | Some (t, (x, ftb)) -> Some (ha :: t, (x, ftb)))
-          | Some (ha, (Some pay, fta)) -> Some ([ha], (Some pay, fta)));;
-
-let rec mynth
-  x0 uu = match x0, uu with [], uu -> None
-    | h :: t, v ->
-        (if equal_nat v zero_nat then h
-          else mynth t (minus_nat (suc (minus_nat v one_nat)) one_nat));;
-
-let rec hexwrite1
-  c = (if equal_nat c zero_nat then '0'
-        else (if equal_nat c one_nat then '1'
-               else (if equal_nat c (nat_of_integer (Big_int.big_int_of_int 2))
-                      then '2'
-                      else (if equal_nat c
-                                 (nat_of_integer (Big_int.big_int_of_int 3))
-                             then '3'
-                             else (if equal_nat c
-(nat_of_integer (Big_int.big_int_of_int 4))
-                                    then '4'
-                                    else (if equal_nat c
-       (nat_of_integer (Big_int.big_int_of_int 5))
-   then '5'
-   else (if equal_nat c (nat_of_integer (Big_int.big_int_of_int 6)) then '6'
-          else (if equal_nat c (nat_of_integer (Big_int.big_int_of_int 7))
-                 then '7'
-                 else (if equal_nat c
-                            (nat_of_integer (Big_int.big_int_of_int 8))
-                        then '8'
-                        else (if equal_nat c
-                                   (nat_of_integer (Big_int.big_int_of_int 9))
-                               then '9'
-                               else (if equal_nat c
-  (nat_of_integer (Big_int.big_int_of_int 10))
-                                      then 'a'
-                                      else (if equal_nat c
-         (nat_of_integer (Big_int.big_int_of_int 11))
-     then 'b'
-     else (if equal_nat c (nat_of_integer (Big_int.big_int_of_int 12)) then 'c'
-            else (if equal_nat c (nat_of_integer (Big_int.big_int_of_int 13))
-                   then 'd'
-                   else (if equal_nat c
-                              (nat_of_integer (Big_int.big_int_of_int 14))
-                          then 'e'
-                          else (if equal_nat c
-                                     (nat_of_integer
-                                       (Big_int.big_int_of_int 15))
-                                 then 'f'
-                                 else failwith "undefined"))))))))))))))));;
-
-let rec hexwrite2
-  w = (let (d, m) =
-         divmod_nat (unat (len0_bit0 (len0_bit0 (len0_bit0 len0_num1))) w)
-           (nat_of_integer (Big_int.big_int_of_int 16))
-         in
-        (hexwrite1 d, hexwrite1 m));;
-
-let rec hexwrite
-  = function [] -> []
-    | h :: t -> (let (c1, c2) = hexwrite2 h in c1 :: c2 :: hexwrite t);;
-
-let rec nat_of_char
-  x = comp nat_of_integer (fun a -> Big_int.big_int_of_int (Char.code a)) x;;
+let rec nat_of_integer
+  k = (if Big_int.le_big_int k Big_int.zero_big_int then Zero_nat
+        else (let (l, j) = divmod_integer k (Big_int.big_int_of_int 2) in
+              let la = nat_of_integer l in
+              let lb = plus_nat la la in
+               (if Big_int.eq_big_int j Big_int.zero_big_int then lb
+                 else plus_nat lb one_nat)));;
 
 let rec truncate_string_sub
   x0 n = match x0, n with
     [], n ->
-      (if equal_nat n zero_nat then []
-        else byteFromNat zero_nat ::
+      (if equal_nata n Zero_nat then []
+        else byteFromNat Zero_nat ::
                truncate_string_sub [] (minus_nat n one_nat))
     | h :: t, n ->
-        (if equal_nat n zero_nat then []
-          else byteFromNat (nat_of_char h) ::
+        (if equal_nata n Zero_nat then []
+          else byteFromNat (nat_of_integer (integer_of_char h)) ::
                  truncate_string_sub t (minus_nat n one_nat));;
 
 let rec truncate_string
-  s = truncate_string_sub s (nat_of_integer (Big_int.big_int_of_int 32));;
+  s = truncate_string_sub s
+        (nat_of_num (Bit0 (Bit0 (Bit0 (Bit0 (Bit0 One))))));;
 
 let rec llll_compile
   = function L4L_Str s -> L (Stack (PUSH_N (truncate_string s)))
-    | L4L_Nat i -> L (Stack (PUSH_N (intToBytes (int_of_nat i))))
+    | L4L_Int i -> L (Stack (PUSH_N (intToBytes i)))
     | L4I0 i -> L i
     | L4I1 (i, l) -> LSeq [llll_compile l; L i]
     | L4I2 (i, l1, l2) -> LSeq [llll_compile l2; llll_compile l1; L i]
+    | L4I3 (i, l1, l2, l3) ->
+        LSeq [llll_compile l3; llll_compile l2; llll_compile l1; L i]
+    | L4I4 (i, l1, l2, l3, l4) ->
+        LSeq [llll_compile l4; llll_compile l3; llll_compile l2;
+               llll_compile l1; L i]
+    | L4In (i, ls) -> LSeq (map llll_compile (rev ls) @ [L i])
     | L4Seq l -> LSeq (map llll_compile l)
     | L4When (c, l) ->
-        LSeq [llll_compile c; L (Arith ISZERO); LJmpI zero_nat; llll_compile l;
-               LLab zero_nat]
+        LSeq [llll_compile c; L (Arith ISZERO); LJmpI Zero_nat; llll_compile l;
+               LLab Zero_nat]
+    | L4Unless (c, l) ->
+        LSeq [llll_compile c; LJmpI Zero_nat; llll_compile l; LLab Zero_nat]
     | L4If (c, l1, l2) ->
-        LSeq [LSeq [llll_compile c; LJmpI zero_nat; llll_compile l2;
-                     LJmp one_nat; LLab zero_nat; llll_compile l1;
+        LSeq [LSeq [llll_compile c; LJmpI Zero_nat; llll_compile l2;
+                     LJmp one_nat; LLab Zero_nat; llll_compile l1;
                      LLab one_nat]]
-    | L4While (c, l) ->
-        LSeq [LSeq [LSeq [LLab zero_nat; llll_compile c; LJmpI one_nat;
-                           LJmp (nat_of_integer (Big_int.big_int_of_int 2));
-                           LLab one_nat; llll_compile l; LJmp zero_nat;
-                           LLab (nat_of_integer (Big_int.big_int_of_int 2))]]]
+    | L4For (i, p, post, body) ->
+        LSeq [LSeq [llll_compile i;
+                     LSeq [LLab Zero_nat; llll_compile p; L (Arith ISZERO);
+                            LJmpI one_nat; llll_compile body; llll_compile post;
+                            LJmp Zero_nat];
+                     LLab Zero_nat]]
+    | L4Revert -> LSeq [LLab Zero_nat; LJmp Zero_nat]
     | L4Arith (LAPlus, ls) -> LSeq (map llll_compile (rev ls) @ [L (Arith ADD)])
     | L4Arith (LAExp, ls) -> LSeq (map llll_compile (rev ls) @ [L (Arith EXP)])
     | L4Arith (LADiv, ls) -> LSeq (map llll_compile (rev ls) @ [L (Arith DIV)])
+    | L4Arith (LAMinus, ls) ->
+        LSeq (map llll_compile (rev ls) @ [L (Arith SUB)])
+    | L4Arith (LAOr, ls) ->
+        LSeq (map llll_compile (rev ls) @ [L (Bits Inst_OR)])
+    | L4Arith (LAAnd, ls) ->
+        LSeq (map llll_compile (rev ls) @ [L (Bits Inst_AND)])
+    | L4Arith (LANot, ls) ->
+        LSeq (map llll_compile (rev ls) @ [L (Bits Inst_NOT)])
+    | L4Logic (LLOr, ls) ->
+        (let res = map llll_compile (rev ls) in
+          LSeq (maps makeLogical res @ [L (Bits Inst_OR)]))
+    | L4Logic (LLAnd, ls) ->
+        (let res = map llll_compile (rev ls) in
+          LSeq (maps makeLogical res @ [L (Bits Inst_AND)]))
+    | L4Logic (LLNot, ls) ->
+        LSeq (map llll_compile (rev ls) @ [L (Arith ISZERO)])
     | L4Comp (LCEq, l1, l2) ->
-        LSeq [llll_compile l2; llll_compile l1; L (Arith Inst_EQ)];;
+        LSeq [llll_compile l2; llll_compile l1; L (Arith Inst_EQ)]
+    | L4Comp (LCNeq, l1, l2) ->
+        LSeq [llll_compile l2; llll_compile l1; L (Arith Inst_EQ);
+               L (Arith ISZERO)]
+    | L4Comp (LCGt, l1, l2) ->
+        LSeq [llll_compile l2; llll_compile l1; L (Arith Inst_GT)]
+    | L4Comp (LCGe, l1, l2) ->
+        LSeq [llll_compile l2; llll_compile l1; L (Arith ISZERO);
+               L (Arith Inst_LT)]
+    | L4Comp (LCLt, l1, l2) ->
+        LSeq [llll_compile l2; llll_compile l1; L (Arith Inst_LT)]
+    | L4Comp (LCLe, l1, l2) ->
+        LSeq [llll_compile l2; llll_compile l1; L (Arith ISZERO);
+               L (Arith Inst_GT)];;
+
+let rec index x0 n = match x0, n with [], n -> None
+                | x :: xs, Zero_nat -> Some x
+                | x :: xs, Suc n -> index xs n;;
+
+let rec list_all p x1 = match p, x1 with p, [] -> true
+                   | p, x :: xs -> p x && list_all p xs;;
 
 let rec mypeel
   = function [] -> Some []
@@ -922,9 +1589,19 @@ let rec mypeel
     | Some h :: t ->
         (match mypeel t with None -> None | Some ta -> Some (h :: ta));;
 
-let rec zero_word _A = word_of_int _A zero_int;;
+let rec zero_word _A = word_of_int _A Zero_int;;
 
-let base_interlude_size : nat = nat_of_integer (Big_int.big_int_of_int 9);;
+let rec nat_to_bytes
+  n = (match
+        divmod_nat n
+          (nat_of_num
+            (Bit0 (Bit0 (Bit0 (Bit0 (Bit0 (Bit0 (Bit0 (Bit0 One)))))))))
+        with (Zero_nat, mo) -> [byteFromNat mo]
+        | (Suc na, mo) -> byteFromNat mo :: nat_to_bytes (Suc na));;
+
+let rec output_address n = rev (nat_to_bytes n);;
+
+let base_interlude_size : nat = nat_of_num (Bit1 (Bit0 (Bit0 One)));;
 
 let rec makeInterlude
   startbytes endbytes prelude payload =
@@ -936,19 +1613,10 @@ let rec makeInterlude
                      (plus_nat
                        (plus_nat (plus_nat (ilsz prelude) startbytes) endbytes)
                        base_interlude_size)))] @
-            [Stack (PUSH_N (output_address zero_nat))] @
+            [Stack (PUSH_N (output_address Zero_nat))] @
               [Memory CODECOPY] @
-                [Stack (PUSH_N (output_address zero_nat))] @
+                [Stack (PUSH_N (output_address Zero_nat))] @
                   [Misc RETURN] @ payload;;
-
-let rec codegena
-  = function (uu, La (uv, i)) -> [i]
-    | (uw, LLaba (ux, uy)) -> [Pc JUMPDEST]
-    | (uz, LJmpa (a, va, s)) -> [Stack (PUSH_N (output_address a)); Pc JUMP]
-    | (vb, LJmpIa (a, vc, vd)) -> [Stack (PUSH_N (output_address a)); Pc JUMPI]
-    | (ve, LSeqa (vf, ls)) -> maps codegena ls;;
-
-let rec codegen ls = maps inst_code (codegena ls);;
 
 let rec ll3_bump
   n x1 = match n, x1 with
@@ -973,8 +1641,8 @@ let rec ll3_init = function (x, La (e, i)) -> (x, La (e, i))
 
 let rec ll4_init = function (x, La (e, i)) -> (x, La (e, i))
                    | (x, LLaba (e, idx)) -> (x, LLaba (e, idx))
-                   | (x, LJmpa (e, idx, s)) -> (x, LJmpa (zero_nat, idx, s))
-                   | (x, LJmpIa (e, idx, s)) -> (x, LJmpIa (zero_nat, idx, s))
+                   | (x, LJmpa (e, idx, s)) -> (x, LJmpa (Zero_nat, idx, s))
+                   | (x, LJmpIa (e, idx, s)) -> (x, LJmpIa (Zero_nat, idx, s))
                    | (x, LSeqa (e, ls)) -> (x, LSeqa (e, map ll4_init ls));;
 
 let rec ll_phase1
@@ -985,13 +1653,11 @@ let rec ll_phase1
     | LLab idx, i ->
         (((i, plus_nat i one_nat), LLaba ((), idx)), plus_nat one_nat i)
     | LJmp idx, i ->
-        (((i, plus_nat (nat_of_integer (Big_int.big_int_of_int 2)) i),
-           LJmpa ((), idx, zero_nat)),
-          plus_nat (nat_of_integer (Big_int.big_int_of_int 2)) i)
+        (((i, plus_nat (nat_of_num (Bit0 One)) i), LJmpa ((), idx, Zero_nat)),
+          plus_nat (nat_of_num (Bit0 One)) i)
     | LJmpI idx, i ->
-        (((i, plus_nat (nat_of_integer (Big_int.big_int_of_int 2)) i),
-           LJmpIa ((), idx, zero_nat)),
-          plus_nat (nat_of_integer (Big_int.big_int_of_int 2)) i)
+        (((i, plus_nat (nat_of_num (Bit0 One)) i), LJmpIa ((), idx, Zero_nat)),
+          plus_nat (nat_of_num (Bit0 One)) i)
     | LSeq ls, i ->
         (let (lsa, ia) = ll_phase1_seq ls i in (((i, ia), LSeqa ((), lsa)), ia))
 and ll_phase1_seq
@@ -1001,38 +1667,286 @@ and ll_phase1_seq
                     let (ta, aa) = a in
                      (ha :: ta, aa));;
 
-let rec ll_pass1 l = fst (ll_phase1 l zero_nat);;
+let rec ll_pass1 l = fst (ll_phase1 l Zero_nat);;
+
+let rec inst_code_clean
+  = function
+    Stack (PUSH_N lst) ->
+      (match stack_inst_code (PUSH_N lst) with [] -> None | h :: _ -> Some [h])
+    | Unknown v -> Some (inst_code (Unknown v))
+    | Bits v -> Some (inst_code (Bits v))
+    | Sarith v -> Some (inst_code (Sarith v))
+    | Arith v -> Some (inst_code (Arith v))
+    | Info v -> Some (inst_code (Info v))
+    | Dup v -> Some (inst_code (Dup v))
+    | Memory v -> Some (inst_code (Memory v))
+    | Storage v -> Some (inst_code (Storage v))
+    | Pc v -> Some (inst_code (Pc v))
+    | Stack POP -> Some (inst_code (Stack POP))
+    | Stack CALLDATALOAD -> Some (inst_code (Stack CALLDATALOAD))
+    | Swap v -> Some (inst_code (Swap v))
+    | Log v -> Some (inst_code (Log v))
+    | Misc v -> Some (inst_code (Misc v));;
+
+let rec codegen_clean
+  = function [] -> Some []
+    | h :: t ->
+        (match inst_code_clean h with None -> None
+          | Some wl ->
+            (match codegen_clean t with None -> None
+              | Some wls -> Some (wl @ wls)));;
+
+let rec ellecompilev_il_wl il = codegen_clean il;;
+
+let rec program_content
+  (Program_ext (program_content, program_length, more)) = program_content;;
+
+let rec get_instsa
+  p start tot =
+    (if less_eq_int tot Zero_int then Some []
+      else (match program_content p start with None -> None
+             | Some i ->
+               (match
+                 get_instsa p (plus_inta start one_inta)
+                   (minus_int tot one_inta)
+                 with None -> None | Some il -> Some (i :: il))));;
+
+let rec cctx_program
+  (Constant_ctx_ext (cctx_program, cctx_this, cctx_hash_filter, more)) =
+    cctx_program;;
+
+let rec program_length
+  (Program_ext (program_content, program_length, more)) = program_length;;
+
+let rec get_insts
+  c = get_instsa (cctx_program c) Zero_int (program_length (cctx_program c));;
+
+let rec ellecompilev_cc_il c = get_insts c;;
+
+let rec program_list_of_lst_validate
+  = function [] -> Some []
+    | Stack (PUSH_N bytes) :: rest ->
+        (if less_eq_nat (size_list bytes) Zero_nat then None
+          else (if less_nat (nat_of_num (Bit0 (Bit0 (Bit0 (Bit0 (Bit0 One))))))
+                     (size_list bytes)
+                 then None
+                 else (match program_list_of_lst_validate rest with None -> None
+                        | Some resta ->
+                          Some ([Stack (PUSH_N bytes)] @
+                                 map (fun a -> Unknown a) bytes @ resta))))
+    | Unknown v :: rest ->
+        (match program_list_of_lst_validate rest with None -> None
+          | Some resta -> Some (Unknown v :: resta))
+    | Bits v :: rest ->
+        (match program_list_of_lst_validate rest with None -> None
+          | Some resta -> Some (Bits v :: resta))
+    | Sarith v :: rest ->
+        (match program_list_of_lst_validate rest with None -> None
+          | Some resta -> Some (Sarith v :: resta))
+    | Arith v :: rest ->
+        (match program_list_of_lst_validate rest with None -> None
+          | Some resta -> Some (Arith v :: resta))
+    | Info v :: rest ->
+        (match program_list_of_lst_validate rest with None -> None
+          | Some resta -> Some (Info v :: resta))
+    | Dup v :: rest ->
+        (match program_list_of_lst_validate rest with None -> None
+          | Some resta -> Some (Dup v :: resta))
+    | Memory v :: rest ->
+        (match program_list_of_lst_validate rest with None -> None
+          | Some resta -> Some (Memory v :: resta))
+    | Storage v :: rest ->
+        (match program_list_of_lst_validate rest with None -> None
+          | Some resta -> Some (Storage v :: resta))
+    | Pc v :: rest ->
+        (match program_list_of_lst_validate rest with None -> None
+          | Some resta -> Some (Pc v :: resta))
+    | Stack POP :: rest ->
+        (match program_list_of_lst_validate rest with None -> None
+          | Some resta -> Some (Stack POP :: resta))
+    | Stack CALLDATALOAD :: rest ->
+        (match program_list_of_lst_validate rest with None -> None
+          | Some resta -> Some (Stack CALLDATALOAD :: resta))
+    | Swap v :: rest ->
+        (match program_list_of_lst_validate rest with None -> None
+          | Some resta -> Some (Swap v :: resta))
+    | Log v :: rest ->
+        (match program_list_of_lst_validate rest with None -> None
+          | Some resta -> Some (Log v :: resta))
+    | Misc v :: rest ->
+        (match program_list_of_lst_validate rest with None -> None
+          | Some resta -> Some (Misc v :: resta));;
+
+let rec cctx_program_update
+  cctx_programa
+    (Constant_ctx_ext (cctx_program, cctx_this, cctx_hash_filter, more)) =
+    Constant_ctx_ext
+      (cctx_programa cctx_program, cctx_this, cctx_hash_filter, more);;
+
+let rec codegen_check
+  = function (uu, La (uv, i)) -> Some [i]
+    | (uw, LLaba (ux, uy)) -> Some [Pc JUMPDEST]
+    | (uz, LJmpa (a, va, s)) ->
+        (if equal_nata (size_list (output_address a)) s
+          then Some [Stack (PUSH_N (output_address a)); Pc JUMP] else None)
+    | (vb, LJmpIa (a, vc, s)) ->
+        (if equal_nata (size_list (output_address a)) s
+          then Some [Stack (PUSH_N (output_address a)); Pc JUMPI] else None)
+    | (vd, LSeqa (ve, ls)) ->
+        (match those (map codegen_check ls) with None -> None
+          | Some lsa -> Some (concat lsa));;
+
+let rec ll4_load_lst_validate
+  cc t =
+    (match codegen_check t with None -> None
+      | Some tc ->
+        (match program_list_of_lst_validate tc with None -> None
+          | Some l ->
+            Some (cctx_program_update
+                   (fun _ ->
+                     make (fun i -> index l (nat i))
+                       (of_nat semiring_1_int (size_list l)))
+                   cc)));;
+
+let rec store_byte_list_in_program
+  uu x1 orig = match uu, x1, orig with uu, [], orig -> orig
+    | pos, h :: t, orig ->
+        store_byte_list_in_program (plus_inta pos one_inta) t
+          (update (equal_int, linorder_int) pos (Unknown h) orig);;
+
+let rec program_avl_of_lst
+  uu x1 = match uu, x1 with uu, [] -> Leaf
+    | pos, Stack (PUSH_N bytes) :: rest ->
+        store_byte_list_in_program (plus_inta pos one_inta) bytes
+          (update (equal_int, linorder_int) pos (Stack (PUSH_N bytes))
+            (program_avl_of_lst
+              (plus_inta (plus_inta pos one_inta)
+                (of_nat semiring_1_int (size_list bytes)))
+              rest))
+    | pos, Unknown v :: rest ->
+        update (equal_int, linorder_int) pos (Unknown v)
+          (program_avl_of_lst (plus_inta pos one_inta) rest)
+    | pos, Bits v :: rest ->
+        update (equal_int, linorder_int) pos (Bits v)
+          (program_avl_of_lst (plus_inta pos one_inta) rest)
+    | pos, Sarith v :: rest ->
+        update (equal_int, linorder_int) pos (Sarith v)
+          (program_avl_of_lst (plus_inta pos one_inta) rest)
+    | pos, Arith v :: rest ->
+        update (equal_int, linorder_int) pos (Arith v)
+          (program_avl_of_lst (plus_inta pos one_inta) rest)
+    | pos, Info v :: rest ->
+        update (equal_int, linorder_int) pos (Info v)
+          (program_avl_of_lst (plus_inta pos one_inta) rest)
+    | pos, Dup v :: rest ->
+        update (equal_int, linorder_int) pos (Dup v)
+          (program_avl_of_lst (plus_inta pos one_inta) rest)
+    | pos, Memory v :: rest ->
+        update (equal_int, linorder_int) pos (Memory v)
+          (program_avl_of_lst (plus_inta pos one_inta) rest)
+    | pos, Storage v :: rest ->
+        update (equal_int, linorder_int) pos (Storage v)
+          (program_avl_of_lst (plus_inta pos one_inta) rest)
+    | pos, Pc v :: rest ->
+        update (equal_int, linorder_int) pos (Pc v)
+          (program_avl_of_lst (plus_inta pos one_inta) rest)
+    | pos, Stack POP :: rest ->
+        update (equal_int, linorder_int) pos (Stack POP)
+          (program_avl_of_lst (plus_inta pos one_inta) rest)
+    | pos, Stack CALLDATALOAD :: rest ->
+        update (equal_int, linorder_int) pos (Stack CALLDATALOAD)
+          (program_avl_of_lst (plus_inta pos one_inta) rest)
+    | pos, Swap v :: rest ->
+        update (equal_int, linorder_int) pos (Swap v)
+          (program_avl_of_lst (plus_inta pos one_inta) rest)
+    | pos, Log v :: rest ->
+        update (equal_int, linorder_int) pos (Log v)
+          (program_avl_of_lst (plus_inta pos one_inta) rest)
+    | pos, Misc v :: rest ->
+        update (equal_int, linorder_int) pos (Misc v)
+          (program_avl_of_lst (plus_inta pos one_inta) rest);;
+
+let rec prog_init_cctx
+  p = Constant_ctx_ext
+        (program_of_lst p
+           (fun lst ->
+             lookup (equal_int, linorder_int)
+               (program_avl_of_lst Zero_int lst)),
+          w160_0, (fun _ -> false), ());;
+
+let rec ellecompilev_4_cc l = ll4_load_lst_validate (prog_init_cctx []) l;;
+
+let rec ll_get_node
+  t x1 = match t, x1 with t, [] -> Some t
+    | (q, LSeqa (e, ls)), v :: va -> ll_get_node_list ls (v :: va)
+    | (vb, La (vd, ve)), v :: va -> None
+    | (vb, LLaba (vd, ve)), v :: va -> None
+    | (vb, LJmpa (vd, ve, vf)), v :: va -> None
+    | (vb, LJmpIa (vd, ve, vf)), v :: va -> None
+and ll_get_node_list
+  uw x1 = match uw, x1 with uw, [] -> None
+    | [], v :: va -> None
+    | h :: ls, Zero_nat :: p -> ll_get_node h p
+    | uy :: ls, Suc v :: p ->
+        ll_get_node_list ls (minus_nat (Suc v) one_nat :: p);;
+
+let rec ll4_validate_jump_targets
+  ns x1 = match ns, x1 with
+    ns, ((xa, x), LJmpa (a, idx, sz)) ->
+      (match mynth ns idx with None -> false | Some b -> equal_nata a b)
+    | ns, ((xa, x), LJmpIa (a, idx, sz)) ->
+        (match mynth ns idx with None -> false | Some b -> equal_nata a b)
+    | ns, (q, LSeqa ([], lsdec)) ->
+        list_all (ll4_validate_jump_targets (None :: ns)) lsdec
+    | ns, (q, LSeqa (v :: va, lsdec)) ->
+        (match ll_get_node (q, LSeqa (v :: va, lsdec)) (v :: va)
+          with None -> false | Some ((_, _), La (_, _)) -> false
+          | Some ((qa, _), LLaba (_, idx)) ->
+            equal_nata (plus_nat idx one_nat) (size_list (v :: va)) &&
+              list_all (ll4_validate_jump_targets (Some qa :: ns)) lsdec
+          | Some ((_, _), LJmpa (_, _, _)) -> false
+          | Some ((_, _), LJmpIa (_, _, _)) -> false
+          | Some ((_, _), LSeqa (_, _)) -> false)
+    | uu, (v, La (vb, vc)) -> true
+    | uu, (v, LLaba (vb, vc)) -> true;;
+
+let rec get_process_jumps_fuela
+  = function
+    (uu, LJmpa (uv, uw, s)) ->
+      minus_nat (nat_of_num (Bit0 (Bit0 (Bit0 (Bit0 (Bit0 One)))))) s
+    | (ux, LJmpIa (uy, uz, s)) ->
+        minus_nat (nat_of_num (Bit0 (Bit0 (Bit0 (Bit0 (Bit0 One)))))) s
+    | (va, LSeqa (vb, ls)) ->
+        foldl (fun a x -> plus_nat a (get_process_jumps_fuela x)) Zero_nat ls
+    | (v, La (vb, vd)) -> Zero_nat
+    | (v, LLaba (vb, vd)) -> Zero_nat;;
+
+let rec get_process_jumps_fuel
+  l = plus_nat one_nat (get_process_jumps_fuela l);;
 
 let rec ll_get_label
-  vd ve = match vd, ve with [], ve -> None
+  vd ve = match vd, ve with
+    ((x, uu), LLaba (uv, uw)) :: ux, [Zero_nat] -> Some x
+    | (uy, LSeqa (uz, lsdec)) :: ls, Zero_nat :: p -> ll_get_label lsdec p
+    | (v, La (vd, ve)) :: ls, Zero_nat :: vb -> None
+    | (v, LJmpa (vd, ve, vf)) :: ls, Zero_nat :: vb -> None
+    | (v, LJmpIa (vd, ve, vf)) :: ls, Zero_nat :: vb -> None
+    | (vb, LLaba (ve, vf)) :: ls, Zero_nat :: v :: vc -> None
+    | (v, La (vb, vd)) :: ls, Suc va :: p ->
+        ll_get_label ls (minus_nat (Suc va) one_nat :: p)
+    | (v, LJmpa (vb, vd, ve)) :: ls, Suc va :: p ->
+        ll_get_label ls (minus_nat (Suc va) one_nat :: p)
+    | (v, LJmpIa (vb, vd, ve)) :: ls, Suc va :: p ->
+        ll_get_label ls (minus_nat (Suc va) one_nat :: p)
+    | (v, LSeqa (vb, vd)) :: ls, Suc va :: p ->
+        ll_get_label ls (minus_nat (Suc va) one_nat :: p)
+    | vc :: ls, Suc v :: p -> ll_get_label ls (minus_nat (Suc v) one_nat :: p)
+    | [], ve -> None
     | (vb, La (vf, vg)) :: va, [] -> None
     | (vb, LJmpa (vf, vg, vh)) :: va, [] -> None
     | (vb, LJmpIa (vf, vg, vh)) :: va, [] -> None
     | (vb, LSeqa (vf, vg)) :: va, [] -> None
-    | vd, [] -> None
-    | (v, La (vd, ve)) :: ls, va :: vb ->
-        (if equal_nat va zero_nat then None
-          else ll_get_label ls
-                 (minus_nat (suc (minus_nat va one_nat)) one_nat :: vb))
-    | (v, LJmpa (vd, ve, vf)) :: ls, va :: vb ->
-        (if equal_nat va zero_nat then None
-          else ll_get_label ls
-                 (minus_nat (suc (minus_nat va one_nat)) one_nat :: vb))
-    | (v, LJmpIa (vd, ve, vf)) :: ls, va :: vb ->
-        (if equal_nat va zero_nat then None
-          else ll_get_label ls
-                 (minus_nat (suc (minus_nat va one_nat)) one_nat :: vb))
-    | (uy, LSeqa (uz, lsdec)) :: ls, va :: p ->
-        (if equal_nat va zero_nat then ll_get_label lsdec p
-          else ll_get_label ls
-                 (minus_nat (suc (minus_nat va one_nat)) one_nat :: p))
-    | ((x, uu), LLaba (uv, uw)) :: ux, [v] ->
-        (if equal_nat v zero_nat then Some x
-          else ll_get_label ux [minus_nat (suc (minus_nat v one_nat)) one_nat])
-    | (vb, LLaba (ve, vf)) :: ls, v :: va :: vc ->
-        (if equal_nat v zero_nat then None
-          else ll_get_label ls
-                 (minus_nat (suc (minus_nat v one_nat)) one_nat :: va :: vc));;
+    | vd, [] -> None;;
 
 let rec write_jump_targets
   ns x1 = match ns, x1 with
@@ -1054,49 +1968,48 @@ let rec write_jump_targets
     | uw, (v, La (vb, vc)) -> Some (v, La (vb, vc))
     | uw, (v, LLaba (vb, vc)) -> Some (v, LLaba (vb, vc));;
 
-let rec encode_size n = plus_nat (nat (log256floor (int_of_nat n))) one_nat;;
+let rec encode_size
+  n = plus_nat (nat (log256floor (of_nat semiring_1_int n))) one_nat;;
 
 let rec ll3_resolve_jump
   x0 oaddr n rel absol = match x0, oaddr, n, rel, absol with
     (uu, LJmpa (e, idx, s)) :: ls, None, n, rel, absol ->
-      (if equal_nat (plus_nat idx one_nat) (size_list rel)
-        then JFail (n :: absol)
+      (if equal_nata idx (size_list rel) then JFail (n :: absol)
         else ll3_resolve_jump ls None (plus_nat n one_nat) rel absol)
     | (uv, LJmpa (e, idx, s)) :: ls, Some addr, n, rel, absol ->
-        (if equal_nat idx (size_list rel)
+        (if equal_nata idx (size_list rel)
           then (if less_nat s (encode_size addr) then JBump (n :: absol)
-                 else (if equal_nat s (encode_size addr)
+                 else (if equal_nata s (encode_size addr)
                         then ll3_resolve_jump ls (Some addr)
                                (plus_nat n one_nat) rel absol
                         else JFail (n :: absol)))
           else ll3_resolve_jump ls (Some addr) (plus_nat n one_nat) rel absol)
     | (uw, LJmpIa (e, idx, s)) :: ls, None, n, rel, absol ->
-        (if equal_nat (plus_nat idx one_nat) (size_list rel)
-          then JFail (n :: absol)
+        (if equal_nata idx (size_list rel) then JFail (n :: absol)
           else ll3_resolve_jump ls None (plus_nat n one_nat) rel absol)
     | (ux, LJmpIa (e, idx, s)) :: ls, Some addr, n, rel, absol ->
-        (if equal_nat idx (size_list rel)
+        (if equal_nata idx (size_list rel)
           then (if less_nat s (encode_size addr) then JBump (n :: absol)
-                 else (if equal_nat s (encode_size addr)
+                 else (if equal_nata s (encode_size addr)
                         then ll3_resolve_jump ls (Some addr)
                                (plus_nat n one_nat) rel absol
                         else JFail (n :: absol)))
           else ll3_resolve_jump ls (Some addr) (plus_nat n one_nat) rel absol)
     | (uy, LSeqa ([], lsdec)) :: ls, oaddr, n, rel, absol ->
-        (match ll3_resolve_jump lsdec oaddr zero_nat (n :: rel) (n :: absol)
+        (match ll3_resolve_jump lsdec oaddr Zero_nat (n :: rel) (n :: absol)
           with JSuccess ->
-            (match ll3_resolve_jump lsdec None zero_nat [] (n :: absol)
+            (match ll3_resolve_jump lsdec None Zero_nat [] (n :: absol)
               with JSuccess ->
                 ll3_resolve_jump ls oaddr (plus_nat n one_nat) rel absol
               | JFail a -> JFail a | JBump a -> JBump a)
           | JFail a -> JFail a | JBump a -> JBump a)
     | (uz, LSeqa (v :: va, lsdec)) :: ls, oaddr, n, rel, absol ->
-        (match ll3_resolve_jump lsdec oaddr zero_nat (n :: rel) (n :: absol)
+        (match ll3_resolve_jump lsdec oaddr Zero_nat (n :: rel) (n :: absol)
           with JSuccess ->
             (match ll_get_label lsdec (v :: va) with None -> JFail absol
               | Some newaddr ->
                 (match
-                  ll3_resolve_jump lsdec (Some newaddr) zero_nat [] (n :: absol)
+                  ll3_resolve_jump lsdec (Some newaddr) Zero_nat [] (n :: absol)
                   with JSuccess ->
                     ll3_resolve_jump ls oaddr (plus_nat n one_nat) rel absol
                   | JFail a -> JFail a | JBump a -> JBump a))
@@ -1110,10 +2023,10 @@ let rec ll3_resolve_jump
 let rec ll3_resolve_jump_wrap
   = function
     (x, LSeqa (e, lsdec)) ->
-      (match e with [] -> ll3_resolve_jump lsdec None zero_nat [] []
+      (match e with [] -> ll3_resolve_jump lsdec None Zero_nat [] []
         | a :: lista ->
           (match ll_get_label lsdec (a :: lista) with None -> JFail []
-            | Some aa -> ll3_resolve_jump lsdec (Some aa) zero_nat [] []))
+            | Some aa -> ll3_resolve_jump lsdec (Some aa) Zero_nat [] []))
     | (v, La (vb, vc)) -> JFail []
     | (v, LLaba (vb, vc)) -> JFail []
     | (v, LJmpa (vb, vc, vd)) -> JFail []
@@ -1122,14 +2035,14 @@ let rec ll3_resolve_jump_wrap
 let rec ll3_inc_jump
   x0 n c = match x0, n, c with
     ((xa, x), LJmpa (e, idx, s)) :: ls, n, [c] ->
-      (if equal_nat n c
+      (if equal_nata n c
         then (((xa, plus_nat x one_nat), LJmpa (e, idx, plus_nat s one_nat)) ::
                 ll3_bump one_nat ls,
                true)
         else (let (lsa, a) = ll3_inc_jump ls (plus_nat n one_nat) [c] in
                (((xa, x), LJmpa (e, idx, s)) :: lsa, a)))
     | ((xa, x), LJmpIa (e, idx, s)) :: ls, n, [c] ->
-        (if equal_nat n c
+        (if equal_nata n c
           then (((xa, plus_nat x one_nat),
                   LJmpIa (e, idx, plus_nat s one_nat)) ::
                   ll3_bump one_nat ls,
@@ -1137,8 +2050,8 @@ let rec ll3_inc_jump
           else (let (lsa, a) = ll3_inc_jump ls (plus_nat n one_nat) [c] in
                  (((xa, x), LJmpIa (e, idx, s)) :: lsa, a)))
     | ((xa, x), LSeqa (e, lsdec)) :: ls, n, c :: cs ->
-        (if equal_nat n c
-          then (match ll3_inc_jump lsdec zero_nat cs
+        (if equal_nata n c
+          then (match ll3_inc_jump lsdec Zero_nat cs
                  with (lsdeca, true) ->
                    (((xa, plus_nat x one_nat), LSeqa (e, lsdeca)) ::
                       ll3_bump one_nat ls,
@@ -1174,7 +2087,7 @@ let rec ll3_inc_jump
 let rec ll3_inc_jump_wrap
   x0 c = match x0, c with
     ((xa, x), LSeqa (e, lsdec)), c ->
-      (match ll3_inc_jump lsdec zero_nat c
+      (match ll3_inc_jump lsdec Zero_nat c
         with (lsdeca, true) -> ((xa, plus_nat x one_nat), LSeqa (e, lsdeca))
         | (_, false) -> ((xa, x), LSeqa (e, lsdec)))
     | (v, La (vb, vc)), uu -> (v, La (vb, vc))
@@ -1183,31 +2096,25 @@ let rec ll3_inc_jump_wrap
     | (v, LJmpIa (vb, vc, vd)), uu -> (v, LJmpIa (vb, vc, vd));;
 
 let rec process_jumps_loop
-  v uu =
-    (if equal_nat v zero_nat then None
-      else (match ll3_resolve_jump_wrap uu with JSuccess -> Some uu
-             | JFail _ -> None
-             | JBump c ->
-               process_jumps_loop
-                 (minus_nat (suc (minus_nat v one_nat)) one_nat)
-                 (ll3_inc_jump_wrap uu (rev c))));;
-
-let rec equal_bool p pa = match p, pa with p, true -> p
-                     | p, false -> not p
-                     | true, p -> p
-                     | false, p -> not p;;
+  x0 uu = match x0, uu with Zero_nat, uu -> None
+    | Suc v, ls ->
+        (match ll3_resolve_jump_wrap ls with JSuccess -> Some ls
+          | JFail _ -> None
+          | JBump c ->
+            process_jumps_loop (minus_nat (Suc v) one_nat)
+              (ll3_inc_jump_wrap ls (rev c)));;
 
 let rec ll3_consume_label
   p n x2 = match p, n, x2 with p, n, [] -> Some ([], [])
     | p, n, (x, LLaba (b, idx)) :: ls ->
-        (if equal_nat idx (size_list p)
+        (if equal_nata idx (size_list p)
           then (if equal_bool b false
                  then Some ((x, LLaba (true, idx)) :: ls, n :: p) else None)
           else (match ll3_consume_label p (plus_nat n one_nat) ls
                  with None -> None
                  | Some (lsa, pa) -> Some ((x, LLaba (b, idx)) :: lsa, pa)))
     | p, n, (x, LSeqa (e, lsdec)) :: ls ->
-        (match ll3_consume_label (n :: p) zero_nat lsdec with None -> None
+        (match ll3_consume_label (n :: p) Zero_nat lsdec with None -> None
           | Some (lsdeca, []) ->
             (match ll3_consume_label p (plus_nat n one_nat) ls with None -> None
               | Some (lsa, pa) -> Some ((x, LSeqa (e, lsdeca)) :: lsa, pa))
@@ -1226,7 +2133,7 @@ let rec ll3_consume_label
 let rec ll3_assign_label
   = function
     (x, LSeqa (e, ls)) ->
-      (match ll3_consume_label [] zero_nat ls with None -> None
+      (match ll3_consume_label [] Zero_nat ls with None -> None
         | Some (lsa, p) ->
           (match ll3_assign_label_list lsa with None -> None
             | Some lsb -> Some (x, LSeqa (rev p, lsb))))
@@ -1243,36 +2150,67 @@ and ll3_assign_label_list
             (match ll3_assign_label_list t with None -> None
               | Some ta -> Some (ha :: ta)));;
 
-let rec pipelinea
-  l n = (match ll3_assign_label (ll3_init (ll_pass1 l)) with None -> None
-          | Some la ->
-            (match process_jumps_loop n la with None -> None
-              | Some lb ->
-                (match write_jump_targets [] (ll4_init lb) with None -> None
-                  | Some a -> Some a)));;
+let rec ellecompile_untrusted
+  l = (match ll3_assign_label (ll3_init (ll_pass1 l)) with None -> None
+        | Some la ->
+          (match process_jumps_loop (get_process_jumps_fuel la) la
+            with None -> None
+            | Some lb ->
+              (match write_jump_targets [] (ll4_init lb) with None -> None
+                | Some a -> Some a)));;
 
-let rec pipeline
-  l n = (match pipelinea l n with None -> None | Some la -> Some (codegen la));;
+let rec gather_ll3_labels_list
+  x0 vp vq vr = match x0, vp, vq, vr with [], vp, vq, vr -> []
+    | h :: t, cp, ofs, d ->
+        gather_ll3_labels h (cp @ [ofs]) d @
+          gather_ll3_labels_list t cp (plus_nat ofs one_nat) d
+and gather_ll3_labels
+  x0 ux uy = match x0, ux, uy with (uu, La (uv, uw)), ux, uy -> []
+    | (uz, LJmpa (va, vb, vc)), vd, ve -> []
+    | (vf, LJmpIa (vg, vh, vi)), vj, vk -> []
+    | (vl, LLaba (vm, n)), cp, d -> (if equal_nata n d then [cp] else [])
+    | (vn, LSeqa (vo, ls)), cp, d ->
+        gather_ll3_labels_list ls cp Zero_nat (plus_nat d one_nat);;
 
-let rec get_process_jumps_fuela
-  = function
-    (uu, LJmpa (uv, uw, s)) ->
-      minus_nat (nat_of_integer (Big_int.big_int_of_int 32)) s
-    | (ux, LJmpIa (uy, uz, s)) ->
-        minus_nat (nat_of_integer (Big_int.big_int_of_int 32)) s
-    | (va, LSeqa (vb, ls)) ->
-        foldl (fun a x -> plus_nat a (get_process_jumps_fuela x)) zero_nat ls
-    | (v, La (vb, vd)) -> zero_nat
-    | (v, LLaba (vb, vd)) -> zero_nat;;
+let rec check_ll3
+  = function (uu, La (uv, uw)) -> true
+    | (ux, LJmpa (uy, uz, va)) -> true
+    | (vb, LJmpIa (vc, vd, ve)) -> true
+    | (vf, LLaba (b, n)) -> equal_bool b true
+    | (vg, LSeqa ([], ls)) ->
+        list_all check_ll3 ls &&
+          null (gather_ll3_labels_list ls [] Zero_nat Zero_nat)
+    | (vh, LSeqa (v :: va, ls)) ->
+        list_all check_ll3 ls &&
+          equal_lista (equal_list equal_nat)
+            (gather_ll3_labels_list ls [] Zero_nat Zero_nat) [v :: va];;
 
-let rec get_process_jumps_fuel
-  l = plus_nat one_nat (get_process_jumps_fuela l);;
+let rec ellecompilev_1_4
+  l = (match ellecompile_untrusted l with None -> None
+        | Some la ->
+          (if check_ll3 la
+            then (if ll4_validate_jump_targets [] la then Some la else None)
+            else None));;
+
+let rec ellecompilev_full
+  l = (match ellecompilev_1_4 l with None -> None
+        | Some l4 ->
+          (match ellecompilev_4_cc l4 with None -> None
+            | Some cc ->
+              (match ellecompilev_cc_il cc with None -> None
+                | Some a -> ellecompilev_il_wl a)));;
+
+let rec ellecompilev_1_il
+  l = (match ellecompilev_1_4 l with None -> None
+        | Some l4 ->
+          (match ellecompilev_4_cc l4 with None -> None
+            | Some a -> ellecompilev_cc_il a));;
 
 let rec llll_combine_payload_sub
   fuel presz paysz startbytes endbytes =
-    (if equal_nat fuel zero_nat then None
-      else (if equal_nat (encode_size paysz) endbytes
-             then (if equal_nat
+    (if equal_nata fuel Zero_nat then None
+      else (if equal_nata (encode_size paysz) endbytes
+             then (if equal_nata
                         (encode_size
                           (plus_nat
                             (plus_nat (plus_nat presz startbytes) endbytes)
@@ -1285,54 +2223,312 @@ let rec llll_combine_payload_sub
                     startbytes (plus_nat endbytes one_nat)));;
 
 let combine_payload_fuel : nat
-  = plus_nat (nat_of_integer (Big_int.big_int_of_int 32))
-      (nat_of_integer (Big_int.big_int_of_int 32));;
+  = plus_nat (nat_of_num (Bit0 (Bit0 (Bit0 (Bit0 (Bit0 One))))))
+      (nat_of_num (Bit0 (Bit0 (Bit0 (Bit0 (Bit0 One))))));;
 
 let default_llll_funs : (char list * (llll list -> llll option)) list
-  = [(['s'; 'e'; 'q'], (fun l -> Some (L4Seq l)));
-      (['i'; 'f'],
+  = [([Chara (true, true, false, false, true, true, true, false);
+        Chara (true, false, true, false, false, true, true, false);
+        Chara (true, false, false, false, true, true, true, false)],
+       (fun l -> Some (L4Seq l)));
+      ([Chara (true, false, false, true, false, true, true, false);
+         Chara (false, true, true, false, false, true, true, false)],
         (fun a ->
           (match a with [] -> None | [_] -> None | [_; _] -> None
             | [c; br1; br2] -> Some (L4If (c, br1, br2))
             | _ :: _ :: _ :: _ :: _ -> None)));
-      (['w'; 'h'; 'e'; 'n'],
+      ([Chara (true, true, true, false, true, true, true, false);
+         Chara (false, false, false, true, false, true, true, false);
+         Chara (true, false, true, false, false, true, true, false);
+         Chara (false, true, true, true, false, true, true, false)],
         (fun a ->
           (match a with [] -> None | [_] -> None
             | [c; br] -> Some (L4When (c, br)) | _ :: _ :: _ :: _ -> None)));
-      (['+'], (fun l -> Some (L4Arith (LAPlus, l))));
-      (['-'], (fun l -> Some (L4Arith (LAMinus, l))));
-      (['*'], (fun l -> Some (L4Arith (LATimes, l))));
-      (['d'; 'i'; 'v'], (fun l -> Some (L4Arith (LADiv, l))));
-      (['e'; 'x'; 'p'], (fun l -> Some (L4Arith (LAExp, l))));
-      (['/'], (fun l -> Some (L4Arith (LADiv, l))));
-      (['%'], (fun l -> Some (L4Arith (LAMod, l))));
-      (['&'], (fun l -> Some (L4Arith (LAAnd, l))));
-      (['|'], (fun l -> Some (L4Arith (LAOr, l))));
-      (['^'], (fun l -> Some (L4Arith (LAXor, l))));
-      (['~'], (fun l -> Some (L4Arith (LANot, l))));
-      (['&'; '&'], (fun l -> Some (L4Logic (LLAnd, l))));
-      (['|'; '|'], (fun l -> Some (L4Logic (LLOr, l))));
-      (['!'], (fun l -> Some (L4Logic (LLNot, l))));
-      (['='],
+      ([Chara (true, false, true, false, true, true, true, false);
+         Chara (false, true, true, true, false, true, true, false);
+         Chara (false, false, true, true, false, true, true, false);
+         Chara (true, false, true, false, false, true, true, false);
+         Chara (true, true, false, false, true, true, true, false);
+         Chara (true, true, false, false, true, true, true, false)],
+        (fun a ->
+          (match a with [] -> None | [_] -> None
+            | [c; br] -> Some (L4Unless (c, br)) | _ :: _ :: _ :: _ -> None)));
+      ([Chara (false, true, true, false, false, true, true, false);
+         Chara (true, true, true, true, false, true, true, false);
+         Chara (false, true, false, false, true, true, true, false)],
+        (fun a ->
+          (match a with [] -> None | [_] -> None | [_; _] -> None
+            | [_; _; _] -> None
+            | [i; p; body; post] -> Some (L4For (i, p, body, post))
+            | _ :: _ :: _ :: _ :: _ :: _ -> None)));
+      ([Chara (true, true, false, true, false, true, false, false)],
+        (fun l -> Some (L4Arith (LAPlus, l))));
+      ([Chara (true, false, false, false, false, true, true, false);
+         Chara (false, false, true, false, false, true, true, false);
+         Chara (false, false, true, false, false, true, true, false)],
+        (fun l -> Some (L4Arith (LAPlus, l))));
+      ([Chara (true, false, true, true, false, true, false, false)],
+        (fun l -> Some (L4Arith (LAMinus, l))));
+      ([Chara (false, true, false, true, false, true, false, false)],
+        (fun l -> Some (L4Arith (LATimes, l))));
+      ([Chara (false, false, true, false, false, true, true, false);
+         Chara (true, false, false, true, false, true, true, false);
+         Chara (false, true, true, false, true, true, true, false)],
+        (fun l -> Some (L4Arith (LADiv, l))));
+      ([Chara (true, false, true, false, false, true, true, false);
+         Chara (false, false, false, true, true, true, true, false);
+         Chara (false, false, false, false, true, true, true, false)],
+        (fun l -> Some (L4Arith (LAExp, l))));
+      ([Chara (true, true, true, true, false, true, false, false)],
+        (fun l -> Some (L4Arith (LADiv, l))));
+      ([Chara (true, false, true, false, false, true, false, false)],
+        (fun l -> Some (L4Arith (LAMod, l))));
+      ([Chara (true, true, false, false, true, true, true, false);
+         Chara (false, false, false, true, false, true, true, false);
+         Chara (true, false, false, false, false, true, true, false);
+         Chara (true, true, false, false, true, true, false, false)],
+        (fun a ->
+          (match a with [] -> None | [_] -> None
+            | [start; width] -> Some (L4I2 (Arith SHA3, start, width))
+            | _ :: _ :: _ :: _ -> None)));
+      ([Chara (true, true, false, true, false, true, true, false);
+         Chara (true, false, true, false, false, true, true, false);
+         Chara (true, true, false, false, false, true, true, false);
+         Chara (true, true, false, false, false, true, true, false);
+         Chara (true, false, false, false, false, true, true, false);
+         Chara (true, true, false, true, false, true, true, false);
+         Chara (false, true, false, false, true, true, false, false);
+         Chara (true, false, true, false, true, true, false, false);
+         Chara (false, true, true, false, true, true, false, false)],
+        (fun a ->
+          (match a with [] -> None | [_] -> None
+            | [start; width] -> Some (L4I2 (Arith SHA3, start, width))
+            | _ :: _ :: _ :: _ -> None)));
+      ([Chara (false, true, true, false, false, true, false, false)],
+        (fun l -> Some (L4Arith (LAAnd, l))));
+      ([Chara (false, false, true, true, true, true, true, false)],
+        (fun l -> Some (L4Arith (LAOr, l))));
+      ([Chara (false, true, true, true, true, false, true, false)],
+        (fun l -> Some (L4Arith (LAXor, l))));
+      ([Chara (false, true, true, true, true, true, true, false)],
+        (fun l -> Some (L4Arith (LANot, l))));
+      ([Chara (true, true, false, false, true, true, true, false);
+         Chara (false, false, false, true, false, true, true, false);
+         Chara (false, true, false, false, true, true, true, false)],
+        (fun a ->
+          (match a with [] -> None | [_] -> None
+            | [vala; shift] ->
+              Some (L4Arith
+                     (LADiv,
+                       [vala;
+                         L4Arith (LAExp, [L4L_Int (Pos (Bit0 One)); shift])]))
+            | _ :: _ :: _ :: _ -> None)));
+      ([Chara (false, true, true, false, false, true, false, false);
+         Chara (false, true, true, false, false, true, false, false)],
+        (fun l -> Some (L4Logic (LLAnd, l))));
+      ([Chara (false, false, true, true, true, true, true, false);
+         Chara (false, false, true, true, true, true, true, false)],
+        (fun l -> Some (L4Logic (LLOr, l))));
+      ([Chara (true, false, false, false, false, true, false, false)],
+        (fun l -> Some (L4Logic (LLNot, l))));
+      ([Chara (true, false, true, true, true, true, false, false)],
         (fun a ->
           (match a with [] -> None | [_] -> None
             | [lhs; rhs] -> Some (L4Comp (LCEq, lhs, rhs))
             | _ :: _ :: _ :: _ -> None)));
-      (['m'; 's'; 't'; 'o'; 'r'; 'e'],
+      ([Chara (true, false, false, false, false, true, false, false);
+         Chara (true, false, true, true, true, true, false, false)],
+        (fun a ->
+          (match a with [] -> None | [_] -> None
+            | [lhs; rhs] -> Some (L4Comp (LCNeq, lhs, rhs))
+            | _ :: _ :: _ :: _ -> None)));
+      ([Chara (false, true, true, true, true, true, false, false)],
+        (fun a ->
+          (match a with [] -> None | [_] -> None
+            | [lhs; rhs] -> Some (L4Comp (LCGt, lhs, rhs))
+            | _ :: _ :: _ :: _ -> None)));
+      ([Chara (false, false, true, true, true, true, false, false)],
+        (fun a ->
+          (match a with [] -> None | [_] -> None
+            | [lhs; rhs] -> Some (L4Comp (LCLt, lhs, rhs))
+            | _ :: _ :: _ :: _ -> None)));
+      ([Chara (false, false, true, true, true, true, false, false);
+         Chara (true, false, true, true, true, true, false, false)],
+        (fun a ->
+          (match a with [] -> None | [_] -> None
+            | [lhs; rhs] -> Some (L4Comp (LCLe, lhs, rhs))
+            | _ :: _ :: _ :: _ -> None)));
+      ([Chara (false, true, true, true, true, true, false, false);
+         Chara (true, false, true, true, true, true, false, false)],
+        (fun a ->
+          (match a with [] -> None | [_] -> None
+            | [lhs; rhs] -> Some (L4Comp (LCGe, lhs, rhs))
+            | _ :: _ :: _ :: _ -> None)));
+      ([Chara (true, false, true, true, false, true, true, false);
+         Chara (true, true, false, false, true, true, true, false);
+         Chara (false, false, true, false, true, true, true, false);
+         Chara (true, true, true, true, false, true, true, false);
+         Chara (false, true, false, false, true, true, true, false);
+         Chara (true, false, true, false, false, true, true, false)],
         (fun a ->
           (match a with [] -> None | [_] -> None
             | [loc; sz] -> Some (L4I2 (Memory MSTORE, loc, sz))
             | _ :: _ :: _ :: _ -> None)));
-      (['r'; 'e'; 't'; 'u'; 'r'; 'n'],
+      ([Chara (true, false, true, true, false, true, true, false);
+         Chara (false, false, true, true, false, true, true, false);
+         Chara (true, true, true, true, false, true, true, false);
+         Chara (true, false, false, false, false, true, true, false);
+         Chara (false, false, true, false, false, true, true, false)],
+        (fun a ->
+          (match a with [] -> None | [loc] -> Some (L4I1 (Memory MLOAD, loc))
+            | _ :: _ :: _ -> None)));
+      ([Chara (false, true, false, false, true, true, true, false);
+         Chara (true, false, true, false, false, true, true, false);
+         Chara (false, false, true, false, true, true, true, false);
+         Chara (true, false, true, false, true, true, true, false);
+         Chara (false, true, false, false, true, true, true, false);
+         Chara (false, true, true, true, false, true, true, false)],
         (fun a ->
           (match a with [] -> None | [_] -> None
             | [loc; sz] -> Some (L4I2 (Misc RETURN, loc, sz))
             | _ :: _ :: _ :: _ -> None)));
-      (['c'; 'a'; 'l'; 'l'; 'd'; 'a'; 't'; 'a'; 'l'; 'o'; 'a'; 'd'],
+      ([Chara (true, true, false, false, true, true, true, false);
+         Chara (false, false, true, false, true, true, true, false);
+         Chara (true, true, true, true, false, true, true, false);
+         Chara (false, false, false, false, true, true, true, false)],
+        (fun _ -> Some (L4I0 (Misc STOP))));
+      ([Chara (true, true, false, false, false, true, true, false);
+         Chara (true, false, false, false, false, true, true, false);
+         Chara (false, false, true, true, false, true, true, false);
+         Chara (false, false, true, true, false, true, true, false);
+         Chara (false, false, true, false, false, true, true, false);
+         Chara (true, false, false, false, false, true, true, false);
+         Chara (false, false, true, false, true, true, true, false);
+         Chara (true, false, false, false, false, true, true, false);
+         Chara (false, false, true, true, false, true, true, false);
+         Chara (true, true, true, true, false, true, true, false);
+         Chara (true, false, false, false, false, true, true, false);
+         Chara (false, false, true, false, false, true, true, false)],
         (fun a ->
           (match a with [] -> None
             | [loc] -> Some (L4I1 (Stack CALLDATALOAD, loc))
-            | _ :: _ :: _ -> None)))];;
+            | _ :: _ :: _ -> None)));
+      ([Chara (true, true, false, false, false, true, true, false);
+         Chara (true, false, false, false, false, true, true, false);
+         Chara (false, false, true, true, false, true, true, false);
+         Chara (false, false, true, true, false, true, true, false);
+         Chara (false, false, true, false, false, true, true, false);
+         Chara (true, false, false, false, false, true, true, false);
+         Chara (false, false, true, false, true, true, true, false);
+         Chara (true, false, false, false, false, true, true, false);
+         Chara (true, true, false, false, false, true, true, false);
+         Chara (true, true, true, true, false, true, true, false);
+         Chara (false, false, false, false, true, true, true, false);
+         Chara (true, false, false, true, true, true, true, false)],
+        (fun a ->
+          (match a with [] -> None | [_] -> None | [_; _] -> None
+            | [dst; src; len] ->
+              Some (L4I3 (Memory CALLDATACOPY, dst, src, len))
+            | _ :: _ :: _ :: _ :: _ -> None)));
+      ([Chara (true, true, false, false, false, true, true, false);
+         Chara (true, false, false, false, false, true, true, false);
+         Chara (false, false, true, true, false, true, true, false);
+         Chara (false, false, true, true, false, true, true, false);
+         Chara (false, false, true, false, false, true, true, false);
+         Chara (true, false, false, false, false, true, true, false);
+         Chara (false, false, true, false, true, true, true, false);
+         Chara (true, false, false, false, false, true, true, false);
+         Chara (true, true, false, false, true, true, true, false);
+         Chara (true, false, false, true, false, true, true, false);
+         Chara (false, true, false, true, true, true, true, false);
+         Chara (true, false, true, false, false, true, true, false)],
+        (fun _ -> Some (L4I0 (Info CALLDATASIZE))));
+      ([Chara (true, true, false, false, false, true, true, false);
+         Chara (true, false, false, false, false, true, true, false);
+         Chara (false, false, true, true, false, true, true, false);
+         Chara (false, false, true, true, false, true, true, false);
+         Chara (false, true, true, false, true, true, true, false);
+         Chara (true, false, false, false, false, true, true, false);
+         Chara (false, false, true, true, false, true, true, false);
+         Chara (true, false, true, false, true, true, true, false);
+         Chara (true, false, true, false, false, true, true, false)],
+        (fun _ -> Some (L4I0 (Info CALLVALUE))));
+      ([Chara (true, true, false, false, false, true, true, false);
+         Chara (true, false, false, false, false, true, true, false);
+         Chara (false, false, true, true, false, true, true, false);
+         Chara (false, false, true, true, false, true, true, false);
+         Chara (true, false, true, false, false, true, true, false);
+         Chara (false, true, false, false, true, true, true, false)],
+        (fun _ -> Some (L4I0 (Info CALLER))));
+      ([Chara (true, true, false, false, true, true, true, false);
+         Chara (true, true, false, false, true, true, true, false);
+         Chara (false, false, true, false, true, true, true, false);
+         Chara (true, true, true, true, false, true, true, false);
+         Chara (false, true, false, false, true, true, true, false);
+         Chara (true, false, true, false, false, true, true, false)],
+        (fun a ->
+          (match a with [] -> None | [_] -> None
+            | [loc; sz] -> Some (L4I2 (Storage SSTORE, loc, sz))
+            | _ :: _ :: _ :: _ -> None)));
+      ([Chara (true, true, false, false, true, true, true, false);
+         Chara (false, false, true, true, false, true, true, false);
+         Chara (true, true, true, true, false, true, true, false);
+         Chara (true, false, false, false, false, true, true, false);
+         Chara (false, false, true, false, false, true, true, false)],
+        (fun [loc] -> Some (L4I1 (Storage SLOAD, loc))));
+      ([Chara (false, false, true, true, false, true, true, false);
+         Chara (true, true, true, true, false, true, true, false);
+         Chara (true, true, true, false, false, true, true, false);
+         Chara (false, false, false, false, true, true, false, false)],
+        (fun l ->
+          (if equal_nata (size_list l) (nat_of_num (Bit0 One))
+            then Some (L4In (Log LOG0, l)) else None)));
+      ([Chara (false, false, true, true, false, true, true, false);
+         Chara (true, true, true, true, false, true, true, false);
+         Chara (true, true, true, false, false, true, true, false);
+         Chara (true, false, false, false, true, true, false, false)],
+        (fun l ->
+          (if equal_nata (size_list l) (nat_of_num (Bit1 One))
+            then Some (L4In (Log LOG1, l)) else None)));
+      ([Chara (false, false, true, true, false, true, true, false);
+         Chara (true, true, true, true, false, true, true, false);
+         Chara (true, true, true, false, false, true, true, false);
+         Chara (false, true, false, false, true, true, false, false)],
+        (fun l ->
+          (if equal_nata (size_list l) (nat_of_num (Bit0 (Bit0 One)))
+            then Some (L4In (Log LOG2, l)) else None)));
+      ([Chara (false, false, true, true, false, true, true, false);
+         Chara (true, true, true, true, false, true, true, false);
+         Chara (true, true, true, false, false, true, true, false);
+         Chara (true, true, false, false, true, true, false, false)],
+        (fun l ->
+          (if equal_nata (size_list l) (nat_of_num (Bit1 (Bit0 One)))
+            then Some (L4In (Log LOG3, l)) else None)));
+      ([Chara (false, false, true, true, false, true, true, false);
+         Chara (true, true, true, true, false, true, true, false);
+         Chara (true, true, true, false, false, true, true, false);
+         Chara (false, false, true, false, true, true, false, false)],
+        (fun l ->
+          (if equal_nata (size_list l) (nat_of_num (Bit0 (Bit1 One)))
+            then Some (L4In (Log LOG4, l)) else None)));
+      ([Chara (false, true, false, false, true, true, true, false);
+         Chara (true, false, true, false, false, true, true, false);
+         Chara (false, true, true, false, true, true, true, false);
+         Chara (true, false, true, false, false, true, true, false);
+         Chara (false, true, false, false, true, true, true, false);
+         Chara (false, false, true, false, true, true, true, false)],
+        (fun _ -> Some L4Revert));
+      ([Chara (false, false, true, true, false, true, true, false);
+         Chara (true, false, false, true, false, true, true, false);
+         Chara (false, false, true, false, true, true, true, false)],
+        (fun a ->
+          (match a with [] -> None | [_] -> None
+            | [loc; lit] ->
+              Some (L4Seq
+                     [lit; L4I0 (Dup (zero_word
+                                       (len0_bit0 (len0_bit0 len0_num1))));
+                       loc; L4I0 (Memory MSTORE)])
+            | _ :: _ :: _ :: _ -> None)))];;
 
 let rec llll_parse1_default
   st = (match llll_parse1 default_llll_funs st with None -> None
@@ -1342,44 +2538,33 @@ let rec llll_parse_complete
   s = (match llll_parse0 s with None -> None
         | Some a -> llll_parse1_default a);;
 
-let rec pipelineb
-  l n = (match pipelinea l n with None -> None
-          | Some la -> Some (codegena la));;
-
 let rec fourL_compiler_string
   s = (match llll_parse_complete s with None -> None
         | Some (l4pre, None) ->
-          (match
-            pipeline (llll_compile l4pre)
-              (get_process_jumps_fuel (ll_pass1 (llll_compile l4pre)))
-            with None -> None | Some wl -> Some (hexwrite wl))
+          (match ellecompilev_full (llll_compile l4pre) with None -> None
+            | Some wl -> Some (hexwrite wl))
         | Some (l4pre, Some l4pay) ->
-          (match
-            pipelineb (llll_compile l4pre)
-              (get_process_jumps_fuel (ll_pass1 (llll_compile l4pre)))
-            with None -> None
+          (match ellecompilev_1_il (llll_compile l4pre) with None -> None
             | Some il_pre ->
-              (match
-                pipelineb (llll_compile l4pay)
-                  (get_process_jumps_fuel (ll_pass1 (llll_compile l4pay)))
-                with None -> None
+              (match ellecompilev_1_il (llll_compile l4pay) with None -> None
                 | Some il_pay ->
                   (match
                     llll_combine_payload_sub combine_payload_fuel (ilsz il_pre)
-                      (ilsz il_pay) zero_nat zero_nat
+                      (ilsz il_pay) Zero_nat Zero_nat
                     with None -> None
                     | Some (startbytes, endbytes) ->
-                      Some (hexwrite
-                             (il2wl
-                               (makeInterlude startbytes endbytes il_pre
-                                 il_pay)))))));;
+                      (match
+                        codegen_clean
+                          (makeInterlude startbytes endbytes il_pre il_pay)
+                        with None -> None | Some wl -> Some (hexwrite wl))))));;
+
+let rec explode
+  s = map char_of_integer
+        (let s = s in let rec exp i l = if i < 0 then l else exp (i - 1) (let k = Char.code (Bytes.get s i) in
+      if k < 128 then Big_int.big_int_of_int k :: l else failwith "Non-ASCII character in literal") in exp (Bytes.length s - 1) []);;
 
 let rec compiler
-  l = (match
-        fourL_compiler_string
-          (let s = l in let rec exp i l = if i < 0 then l else exp (i - 1) (String.get s i :: l) in exp (String.length s - 1) [])
-        with None -> None
-        | Some s ->
-          Some (let l = s in let res = String.create (List.length l) in let rec imp i = function | [] -> res | c :: l -> String.set res i c; imp (i + 1) l in imp 0 l));;
+  l = (match fourL_compiler_string (explode l) with None -> None
+        | Some s -> Some (implode s));;
 
 end;; (*struct FourL*)
