elle/ElleCompiler.thy
@@ -214,7 +214,7 @@ answer: this has now become a separate pre-screening pass *)
 fun ll3_resolve_jump :: "ll3 list \<Rightarrow> nat option \<Rightarrow> nat \<Rightarrow> childpath \<Rightarrow> childpath \<Rightarrow> jump_resolve_result" where
   (* TODO: does this handle returning the childpath correctly? should it be n#c?*)
   "ll3_resolve_jump ((_, LJmp e idx s)#ls) None n rel absol = 
-   (if idx + 1 = length rel then JFail (n#absol)
+   (if idx (*+ 1*) = length rel then JFail (n#absol)
     else ll3_resolve_jump ls None (n+1) rel absol)"
 
 | "ll3_resolve_jump ((_, LJmp e idx s)#ls) (Some addr) n rel absol =
@@ -225,7 +225,7 @@ fun ll3_resolve_jump :: "ll3 list \<Rightarrow> nat option \<Rightarrow> nat \<R
         else ll3_resolve_jump ls (Some addr) (n+1) rel absol)"
 
 |  "ll3_resolve_jump ((_, LJmpI e idx s)#ls) None n rel absol = 
-   (if idx + 1 = length rel then JFail (n#absol)
+   (if idx (*+ 1*) = length rel then JFail (n#absol)
     else ll3_resolve_jump ls None (n+1) rel absol)"
 
 | "ll3_resolve_jump ((_, LJmpI e idx s)#ls) (Some addr) n rel absol =
